Superposition_Calculus/First_Order_Superposition_Completeness.thy
@@ -46,7 +46,7 @@ proof(cases D\<^sub>G C\<^sub>G rule: ground.eq_resolution.cases)
     l_\<gamma>_is_maximal: "?select\<^sub>G_empty \<Longrightarrow> is_maximal (l \<cdot>l \<gamma>) (D \<cdot> \<gamma>)"
   proof-
     obtain max_l where 
-     "is_maximal max_l D" and
+      "is_maximal max_l D" and
       is_max_in_D_\<gamma>: "is_maximal (max_l \<cdot>l \<gamma>) (D \<cdot> \<gamma>)"
     proof-
       have "D \<noteq> {#}"
@@ -125,128 +125,136 @@ proof(cases D\<^sub>G C\<^sub>G rule: ground.eq_resolution.cases)
       by auto
 
     show ?thesis
-      using welltyped_imgu_exists[OF unified welltyped] that
+      using obtain_welltyped_imgu[OF unified welltyped] that
       by metis
   qed
 
-  have eq_resolution: "eq_resolution (D, \<V>) (C' \<cdot> \<mu>, \<V>)"
-  proof (rule eq_resolutionI, rule D, rule l, rule imgu)
-    show "select D = {#} \<and> is_maximal (l \<cdot>l \<mu>) (D \<cdot> \<mu>) \<or> is_maximal (l \<cdot>l \<mu>) ((select D) \<cdot> \<mu>)"
-    proof(cases ?select\<^sub>G_empty)
-      case True
+  show ?thesis
+  proof(rule that)
 
-      moreover have "is_maximal (l \<cdot>l \<mu>) (D \<cdot> \<mu>)"
-      proof-
-        have "l \<cdot>l \<mu> \<in># D \<cdot> \<mu>"
-          using l_in_D 
+    show eq_resolution: "eq_resolution (D, \<V>) (C' \<cdot> \<mu>, \<V>)"
+    proof (rule eq_resolutionI, rule D, rule l, rule imgu)
+      show "select D = {#} \<and> is_maximal (l \<cdot>l \<mu>) (D \<cdot> \<mu>) \<or> is_maximal (l \<cdot>l \<mu>) ((select D) \<cdot> \<mu>)"
+      proof(cases ?select\<^sub>G_empty)
+        case True
+
+        moreover have "is_maximal (l \<cdot>l \<mu>) (D \<cdot> \<mu>)"
+        proof-
+          have "l \<cdot>l \<mu> \<in># D \<cdot> \<mu>"
+            using l_in_D 
+            by blast
+
+          then show ?thesis
+            using l_\<gamma>_is_maximal[OF True] is_maximal_if_grounding_is_maximal D_grounding
+            unfolding \<gamma>
+            by simp
+        qed
+
+        ultimately show ?thesis
+          using select
+          by simp
+      next
+        case False
+
+        have "l \<cdot>l \<mu> \<in># select D \<cdot> \<mu>"
+          using l_selected[OF False] maximal_in_clause
           by blast
 
-        then show ?thesis
-          using l_\<gamma>_is_maximal[OF True] is_maximal_if_grounding_is_maximal D_grounding
+        then have "is_maximal (l \<cdot>l \<mu>) (select D \<cdot> \<mu>)"
+          using 
+            select_ground_subst[OF D_grounding]
+            l_\<gamma>_selected[OF False] 
+            is_maximal_if_grounding_is_maximal 
           unfolding \<gamma>
+          by auto
+
+        then show ?thesis
+          using select
+          by blast
+      qed
+    qed simp
+
+    show C'_\<mu>_\<gamma>: "C' \<cdot> \<mu> \<cdot> \<gamma> = C \<cdot> \<gamma>"
+    proof-
+      have "term.is_idem \<mu>"
+        using imgu 
+        unfolding term_subst.is_imgu_iff_is_idem_and_is_mgu 
+        by blast  
+
+      then have \<mu>_\<gamma>: "\<mu> \<odot> \<gamma> = \<gamma>"
+        unfolding \<gamma> term_subst.is_idem_def subst_compose_assoc[symmetric]
+        by argo
+
+      have "D \<cdot> \<gamma> = add_mset (l \<cdot>l \<gamma>) (C \<cdot> \<gamma>)"
+      proof-
+        have "clause.to_ground (D \<cdot> \<gamma>) = clause.to_ground (add_mset (l \<cdot>l \<gamma>) (C \<cdot> \<gamma>))"
+          using ground_eq_resolutionI(1)
+          unfolding D\<^sub>G ground_eq_resolutionI(2) l_\<gamma> ground_eq_resolutionI(4)[symmetric]
+          by simp 
+
+        moreover have "clause.is_ground (add_mset (l \<cdot>l \<gamma>) (C \<cdot> \<gamma>))"
+          using C_grounding clause.to_set_is_ground_subst[OF l_in_D D_grounding]
           by simp
+
+        ultimately show ?thesis
+          using clause.to_ground_eq[OF D_grounding]
+          by blast
       qed
 
-      ultimately show ?thesis
-        using select
+      then have "C' \<cdot> \<gamma> = C \<cdot> \<gamma>"
+        unfolding D
         by simp
-    next
-      case False
-
-      have "l \<cdot>l \<mu> \<in># select D \<cdot> \<mu>"
-        using l_selected[OF False] maximal_in_clause
-        by blast
-
-      then have "is_maximal (l \<cdot>l \<mu>) (select D \<cdot> \<mu>)"
-        using 
-          select_ground_subst[OF D_grounding]
-          l_\<gamma>_selected[OF False] 
-          is_maximal_if_grounding_is_maximal 
-        unfolding \<gamma>
-        by auto
 
       then show ?thesis
-        using select
-        by blast
+        unfolding clause.subst_comp_subst[symmetric] \<mu>_\<gamma>.
     qed
-  qed simp
 
-  have C_\<gamma>: "C \<cdot> \<gamma> = C' \<cdot> \<mu> \<cdot> \<gamma>"
-  proof-
-    have "term.is_idem \<mu>"
-      using imgu 
-      unfolding term_subst.is_imgu_iff_is_idem_and_is_mgu 
-      by blast  
-
-    then have \<mu>_\<gamma>: "\<mu> \<odot> \<gamma> = \<gamma>"
-      unfolding \<gamma> term_subst.is_idem_def subst_compose_assoc[symmetric]
-      by argo
-
-    have "D \<cdot> \<gamma> = add_mset (l \<cdot>l \<gamma>) (C \<cdot> \<gamma>)"
+    show "Infer [D\<^sub>G] C\<^sub>G \<in> inference_groundings (Infer [(D, \<V>)] (C' \<cdot> \<mu>, \<V>))"
     proof-
-      have "clause.to_ground (D \<cdot> \<gamma>) = clause.to_ground (add_mset (l \<cdot>l \<gamma>) (C \<cdot> \<gamma>))"
-        using ground_eq_resolutionI(1)
-        unfolding D\<^sub>G ground_eq_resolutionI(2) l_\<gamma> ground_eq_resolutionI(4)[symmetric]
-        by simp 
 
-      moreover have "clause.is_ground (add_mset (l \<cdot>l \<gamma>) (C \<cdot> \<gamma>))"
-        using C_grounding clause.to_set_is_ground_subst[OF l_in_D D_grounding]
-        by simp
+      have "is_inference_grounding_one_premise (D, \<V>) (C' \<cdot> \<mu>, \<V>) (Infer [D\<^sub>G] C\<^sub>G) \<gamma>"
+      proof(unfold split, intro conjI; (rule D_grounding D_is_welltyped refl \<V>)?)
+        show "clause.is_ground (C' \<cdot> \<mu> \<cdot> \<gamma>)"
+          using C_grounding C'_\<mu>_\<gamma>
+          by argo
+      next
+        show "Infer [D\<^sub>G] C\<^sub>G = Infer [clause.to_ground (D \<cdot> \<gamma>)] (clause.to_ground (C' \<cdot> \<mu> \<cdot> \<gamma>))"
+          using C'_\<mu>_\<gamma>
+          by simp
+      next
+        have "clause.vars (C' \<cdot> \<mu>) \<subseteq> clause.vars D"
+          using clause.variables_in_base_imgu imgu
+          unfolding D l
+          by auto
+
+        then show "is_welltyped_on (clause.vars (C' \<cdot> \<mu>)) \<V> \<gamma>"
+          using D_is_welltyped \<gamma>_is_welltyped
+          by blast
+      next
+        show "clause.is_welltyped \<V> (C' \<cdot> \<mu>)"
+          using D_is_welltyped eq_resolution eq_resolution_preserves_typing
+          by blast
+      qed
+
+      moreover have "Infer [D\<^sub>G] C\<^sub>G \<in> ground.G_Inf"
+        unfolding ground.G_Inf_def
+        using ground_eq_resolution
+        by blast
 
       ultimately show ?thesis
-        using clause.to_ground_eq[OF D_grounding]
-        by blast
-    qed
-
-    then have "C \<cdot> \<gamma> = C' \<cdot> \<gamma>"
-      unfolding D
-      by simp
-
-    then show ?thesis
-      unfolding clause.subst_comp_subst[symmetric] \<mu>_\<gamma>.
-  qed
- 
-  moreover have "Infer [D\<^sub>G] C\<^sub>G \<in> inference_groundings (Infer [(D, \<V>)] (C' \<cdot> \<mu>, \<V>))"
-  proof-
-
-    have "is_inference_grounding_one_premise (D, \<V>) (C' \<cdot> \<mu>, \<V>) (Infer [D\<^sub>G] C\<^sub>G) \<gamma>"
-    proof(unfold split, intro conjI; (rule D_grounding D_is_welltyped refl \<V>)?)
-      show "clause.is_ground (C' \<cdot> \<mu> \<cdot> \<gamma>)"
-        using C_grounding C_\<gamma> 
-        by argo
-    next
-      show "Infer [D\<^sub>G] C\<^sub>G = Infer [clause.to_ground (D \<cdot> \<gamma>)] (clause.to_ground (C' \<cdot> \<mu> \<cdot> \<gamma>))"
-        using C_\<gamma>
-        by simp
-    next
-      have "clause.vars (C' \<cdot> \<mu>) \<subseteq> clause.vars D"
-        using clause.variables_in_base_imgu imgu
-        unfolding D l
+        unfolding inference_groundings_def
         by auto
-
-      then show "is_welltyped_on (clause.vars (C' \<cdot> \<mu>)) \<V> \<gamma>"
-        using D_is_welltyped \<gamma>_is_welltyped
-        by blast
-    next
-      show "clause.is_welltyped \<V> (C' \<cdot> \<mu>)"
-        using D_is_welltyped eq_resolution eq_resolution_preserves_typing
-        by blast
     qed
-
-    moreover have "Infer [D\<^sub>G] C\<^sub>G \<in> ground.G_Inf"
-      unfolding ground.G_Inf_def
-      using ground_eq_resolution
-      by blast
-
-    ultimately show ?thesis
-      unfolding inference_groundings_def
-      by auto
   qed
-
-  ultimately show ?thesis
-    using that[OF eq_resolution]
-    by presburger
 qed
+
+(* TODO: *)
+lemma move_simp: "{x. if b x then P x else Q x } = 
+        {x. b x \<and> P x } \<union> {x. \<not>b x \<and> Q x}"
+  by auto
+
+lemma zz: "{x. x \<notin> X \<and> P x} = {x. P x} - {x. x \<in> X}"
+  by auto
 
 lemma eq_factoring_lifting:
   fixes 
@@ -359,1016 +367,858 @@ proof(cases D\<^sub>G C\<^sub>G rule: ground.eq_factoring.cases)
       by simp_all
 
     then show ?thesis
-      using welltyped_imgu_exists[OF unified welltyped] that
+      using obtain_welltyped_imgu[OF unified welltyped] that
       by metis
   qed
 
-  let ?C' = "add_mset (t\<^sub>1 \<approx> t\<^sub>2') (add_mset (t\<^sub>1' !\<approx> t\<^sub>2') D')"
+  let ?C'' = "add_mset (t\<^sub>1 \<approx> t\<^sub>2') (add_mset (t\<^sub>1' !\<approx> t\<^sub>2') D')"
+  let ?C' = "?C'' \<cdot> \<mu>"
 
-  have eq_factoring: "eq_factoring (D, \<V>) (?C' \<cdot> \<mu>, \<V>)"
-  proof (rule eq_factoringI; (rule D l\<^sub>1 l\<^sub>2 imgu refl)?)
-    show "select D = {#}"
-      using ground_eq_factoringI(4) select
-      by simp
-  next
-    have "l\<^sub>1 \<cdot>l \<mu> \<in># D \<cdot> \<mu>"
-      using l\<^sub>1_is_maximal clause.subst_in_to_set_subst maximal_in_clause 
-      by blast
+  show ?thesis
+  proof(rule that)
 
-    then show "is_maximal (l\<^sub>1 \<cdot>l \<mu>) (D \<cdot> \<mu>)"
-      using is_maximal_if_grounding_is_maximal D_grounding l\<^sub>1_\<gamma>_is_maximal
-      unfolding \<gamma>
-      by auto
-  next
-    have groundings: "term.is_ground (t\<^sub>1' \<cdot>t \<mu> \<cdot>t \<sigma>)" "term.is_ground (t\<^sub>1 \<cdot>t \<mu> \<cdot>t \<sigma>)"
-      using t\<^sub>1'_\<gamma> t\<^sub>1_\<gamma>
-      unfolding \<gamma>
-      by simp_all
-
-    have "t\<^sub>1' \<cdot>t \<gamma> \<prec>\<^sub>t t\<^sub>1 \<cdot>t \<gamma>"
-      using ground_eq_factoringI(6)
-      unfolding t\<^sub>1'_\<gamma> t\<^sub>1_\<gamma> term.order.less\<^sub>G_def.
-
-    then show "\<not> t\<^sub>1 \<cdot>t \<mu> \<preceq>\<^sub>t t\<^sub>1' \<cdot>t \<mu>"
-      unfolding \<gamma> 
-      using term.order.ground_less_not_less_eq[OF groundings]
-      by simp
-  qed
-
-  have C_\<gamma>: "C \<cdot> \<gamma> = ?C' \<cdot> \<mu> \<cdot> \<gamma>"
-  proof-
-    have "term.is_idem \<mu>"
-      using imgu 
-      unfolding term_subst.is_imgu_iff_is_idem_and_is_mgu 
-      by blast  
-
-    then have \<mu>_\<gamma>: "\<mu> \<odot> \<gamma> = \<gamma>"
-      unfolding \<gamma> term_subst.is_idem_def subst_compose_assoc[symmetric]
-      by argo
-
-    have "C \<cdot> \<gamma> = clause.from_ground (add_mset (t\<^sub>G\<^sub>2 !\<approx> t\<^sub>G\<^sub>3) (add_mset (t\<^sub>G\<^sub>1 \<approx> t\<^sub>G\<^sub>3) D\<^sub>G'))"
-      using ground_eq_factoringI(7) clause.to_ground_eq[OF C_grounding clause.ground_is_ground]
-      unfolding C\<^sub>G
-      by (metis clause.from_ground_inverse)
-
-    also have "... = ?C' \<cdot> \<gamma>"
-      using t\<^sub>1_\<gamma> t\<^sub>1'_\<gamma> t\<^sub>2'_\<gamma> D'_\<gamma>
-      by simp
-
-    also have "... = ?C' \<cdot> \<mu> \<cdot> \<gamma>"
-      unfolding clause.subst_comp_subst[symmetric] \<mu>_\<gamma> ..
-      
-    finally show ?thesis.
-  qed
-
-  moreover have "Infer [D\<^sub>G] C\<^sub>G \<in> inference_groundings (Infer [(D, \<V>)] (?C' \<cdot> \<mu>, \<V>))"
-  proof-
-    have "is_inference_grounding_one_premise (D, \<V>) (?C' \<cdot> \<mu>, \<V>) (Infer [D\<^sub>G] C\<^sub>G) \<gamma>"
-    proof(unfold split, intro conjI; (rule D_grounding D_is_welltyped refl \<V>)?)
-      show "clause.is_ground (?C' \<cdot> \<mu> \<cdot> \<gamma>)"
-        using C_grounding C_\<gamma>
-        by argo
-    next
-      show "Infer [D\<^sub>G] C\<^sub>G = Infer [clause.to_ground (D \<cdot> \<gamma>)] (clause.to_ground (?C' \<cdot> \<mu> \<cdot> \<gamma>))"
-        using C_\<gamma>
+    show eq_factoring: "eq_factoring (D, \<V>) (?C', \<V>)"
+    proof (rule eq_factoringI; (rule D l\<^sub>1 l\<^sub>2 imgu refl)?)
+      show "select D = {#}"
+        using ground_eq_factoringI(4) select
         by simp
     next
-      have imgu: "term.is_imgu \<mu> {{t\<^sub>1, t\<^sub>2}}"
-        using imgu
+      have "l\<^sub>1 \<cdot>l \<mu> \<in># D \<cdot> \<mu>"
+        using l\<^sub>1_is_maximal clause.subst_in_to_set_subst maximal_in_clause 
         by blast
 
-      have "clause.vars (?C' \<cdot> \<mu>) \<subseteq> clause.vars D"
-        using clause.variables_in_base_imgu[OF imgu, of ?C']
-        unfolding D l\<^sub>1 l\<^sub>2
+      then show "is_maximal (l\<^sub>1 \<cdot>l \<mu>) (D \<cdot> \<mu>)"
+        using is_maximal_if_grounding_is_maximal D_grounding l\<^sub>1_\<gamma>_is_maximal
+        unfolding \<gamma>
         by auto
-
-      then show "is_welltyped_on (clause.vars (?C' \<cdot> \<mu>)) \<V> \<gamma>"
-        using D_is_welltyped \<gamma>_is_welltyped
-        by blast
     next
-      show "clause.is_welltyped \<V> (?C' \<cdot> \<mu>)"
-        using D_is_welltyped eq_factoring eq_factoring_preserves_typing
-        by blast
+      have groundings: "term.is_ground (t\<^sub>1' \<cdot>t \<mu> \<cdot>t \<sigma>)" "term.is_ground (t\<^sub>1 \<cdot>t \<mu> \<cdot>t \<sigma>)"
+        using t\<^sub>1'_\<gamma> t\<^sub>1_\<gamma>
+        unfolding \<gamma>
+        by simp_all
+
+      have "t\<^sub>1' \<cdot>t \<gamma> \<prec>\<^sub>t t\<^sub>1 \<cdot>t \<gamma>"
+        using ground_eq_factoringI(6)
+        unfolding t\<^sub>1'_\<gamma> t\<^sub>1_\<gamma> term.order.less\<^sub>G_def.
+
+      then show "\<not> t\<^sub>1 \<cdot>t \<mu> \<preceq>\<^sub>t t\<^sub>1' \<cdot>t \<mu>"
+        unfolding \<gamma> 
+        using term.order.ground_less_not_less_eq[OF groundings]
+        by simp
     qed
 
-    moreover have "Infer [D\<^sub>G] C\<^sub>G \<in> ground.G_Inf"
-      unfolding ground.G_Inf_def
-      using ground_eq_factoring
-      by blast
+    show C'_\<gamma>: "?C' \<cdot> \<gamma> = C \<cdot> \<gamma>"
+    proof-
+      have "term.is_idem \<mu>"
+        using imgu 
+        unfolding term_subst.is_imgu_iff_is_idem_and_is_mgu 
+        by blast  
 
-    ultimately show ?thesis
-      unfolding inference_groundings_def
-      by auto
+      then have \<mu>_\<gamma>: "\<mu> \<odot> \<gamma> = \<gamma>"
+        unfolding \<gamma> term_subst.is_idem_def subst_compose_assoc[symmetric]
+        by argo
+
+      have "C \<cdot> \<gamma> = clause.from_ground (add_mset (t\<^sub>G\<^sub>2 !\<approx> t\<^sub>G\<^sub>3) (add_mset (t\<^sub>G\<^sub>1 \<approx> t\<^sub>G\<^sub>3) D\<^sub>G'))"
+        using ground_eq_factoringI(7) clause.to_ground_eq[OF C_grounding clause.ground_is_ground]
+        unfolding C\<^sub>G
+        by (metis clause.from_ground_inverse)
+
+      also have "... = ?C'' \<cdot> \<gamma>"
+        using t\<^sub>1_\<gamma> t\<^sub>1'_\<gamma> t\<^sub>2'_\<gamma> D'_\<gamma>
+        by simp
+
+      also have "... = ?C' \<cdot> \<gamma>"
+        unfolding clause.subst_comp_subst[symmetric] \<mu>_\<gamma> ..
+
+      finally show ?thesis ..
+    qed
+
+    show "Infer [D\<^sub>G] C\<^sub>G \<in> inference_groundings (Infer [(D, \<V>)] (?C', \<V>))"
+    proof-
+      have "is_inference_grounding_one_premise (D, \<V>) (?C', \<V>) (Infer [D\<^sub>G] C\<^sub>G) \<gamma>"
+      proof(unfold split, intro conjI; (rule D_grounding D_is_welltyped refl \<V>)?)
+        show "clause.is_ground (?C' \<cdot> \<gamma>)"
+          using C_grounding C'_\<gamma>
+          by argo
+      next
+        show "Infer [D\<^sub>G] C\<^sub>G = Infer [clause.to_ground (D \<cdot> \<gamma>)] (clause.to_ground (?C' \<cdot> \<gamma>))"
+          using C'_\<gamma>
+          by simp
+      next
+        have imgu: "term.is_imgu \<mu> {{t\<^sub>1, t\<^sub>2}}"
+          using imgu
+          by blast
+
+        have "clause.vars ?C' \<subseteq> clause.vars D"
+          using clause.variables_in_base_imgu[OF imgu, of ?C'']
+          unfolding D l\<^sub>1 l\<^sub>2
+          by auto
+
+        then show "is_welltyped_on (clause.vars ?C') \<V> \<gamma>"
+          using D_is_welltyped \<gamma>_is_welltyped
+          by blast
+      next
+        show "clause.is_welltyped \<V> ?C'"
+          using D_is_welltyped eq_factoring eq_factoring_preserves_typing
+          by blast
+      qed
+
+      moreover have "Infer [D\<^sub>G] C\<^sub>G \<in> ground.G_Inf"
+        unfolding ground.G_Inf_def
+        using ground_eq_factoring
+        by blast
+
+      ultimately show ?thesis
+        unfolding inference_groundings_def
+        by auto
+    qed
   qed
-
-  ultimately show ?thesis
-    using that[OF eq_factoring]
-    by presburger
 qed
 
 lemma superposition_lifting:
-  fixes 
-    premise\<^sub>G\<^sub>1 premise\<^sub>G\<^sub>2 conclusion\<^sub>G :: "'f gatom clause" and 
-    premise\<^sub>1 premise\<^sub>2 "conclusion" :: "('f, 'v) atom clause" and
+  fixes
+    E\<^sub>G D\<^sub>G C\<^sub>G :: "'f ground_atom clause" and
+    E D C :: "('f, 'v) atom clause" and
     \<gamma> \<rho>\<^sub>1 \<rho>\<^sub>2 :: "('f, 'v) subst" and
-    \<V>\<^sub>1 \<V>\<^sub>2
-  defines 
-    premise\<^sub>G\<^sub>1 [simp]: "premise\<^sub>G\<^sub>1 \<equiv> clause.to_ground (premise\<^sub>1 \<cdot> \<rho>\<^sub>1 \<cdot> \<gamma>)" and
-    premise\<^sub>G\<^sub>2 [simp]: "premise\<^sub>G\<^sub>2 \<equiv> clause.to_ground (premise\<^sub>2 \<cdot> \<rho>\<^sub>2 \<cdot> \<gamma>)" and
-    conclusion\<^sub>G [simp]: "conclusion\<^sub>G \<equiv> clause.to_ground (conclusion \<cdot> \<gamma>)" and
-    premise_groundings [simp]: 
-    "premise_groundings \<equiv> clause_groundings (premise\<^sub>1, \<V>\<^sub>1) \<union> clause_groundings (premise\<^sub>2, \<V>\<^sub>2)" and
-    \<iota>\<^sub>G [simp]: "\<iota>\<^sub>G \<equiv> Infer [premise\<^sub>G\<^sub>2, premise\<^sub>G\<^sub>1] conclusion\<^sub>G"
-  assumes 
-    renaming: 
-    "term_subst.is_renaming \<rho>\<^sub>1" 
-    "term_subst.is_renaming \<rho>\<^sub>2" 
-    "clause.vars (premise\<^sub>1 \<cdot> \<rho>\<^sub>1) \<inter> clause.vars (premise\<^sub>2 \<cdot> \<rho>\<^sub>2) = {}"  and
-    premise\<^sub>1_grounding: "clause.is_ground (premise\<^sub>1 \<cdot> \<rho>\<^sub>1 \<cdot> \<gamma>)" and
-    premise\<^sub>2_grounding: "clause.is_ground (premise\<^sub>2 \<cdot> \<rho>\<^sub>2 \<cdot> \<gamma>)" and
-    conclusion_grounding: "clause.is_ground (conclusion \<cdot> \<gamma>)" and
-    select: 
-    "clause.from_ground (select\<^sub>G premise\<^sub>G\<^sub>1) = (select premise\<^sub>1) \<cdot> \<rho>\<^sub>1 \<cdot> \<gamma>"
-    "clause.from_ground (select\<^sub>G premise\<^sub>G\<^sub>2) = (select premise\<^sub>2) \<cdot> \<rho>\<^sub>2 \<cdot> \<gamma>" and
-    ground_superposition: "ground.superposition premise\<^sub>G\<^sub>2 premise\<^sub>G\<^sub>1 conclusion\<^sub>G" and
-    non_redundant: "\<iota>\<^sub>G \<notin> ground.Red_I premise_groundings" and
-    typing:
-    "clause.is_welltyped \<V>\<^sub>1 premise\<^sub>1"
-    "clause.is_welltyped \<V>\<^sub>2 premise\<^sub>2"
-    (*"term_subst.is_ground_subst \<gamma>"*)
-    "is_welltyped_on (clause.vars premise\<^sub>1) \<V>\<^sub>1 (\<rho>\<^sub>1 \<odot> \<gamma>)"
-    "is_welltyped_on (clause.vars premise\<^sub>2) \<V>\<^sub>2 (\<rho>\<^sub>2 \<odot> \<gamma>)"
-    "is_welltyped_on (clause.vars premise\<^sub>1) \<V>\<^sub>1 \<rho>\<^sub>1"
-    "is_welltyped_on (clause.vars premise\<^sub>2) \<V>\<^sub>2 \<rho>\<^sub>2"
-    "infinite_variables_per_type \<V>\<^sub>1" "infinite_variables_per_type \<V>\<^sub>2"
-  obtains conclusion' \<V>\<^sub>3
+    \<V>\<^sub>1 \<V>\<^sub>2 :: "('v, 'ty) var_types"
+  defines
+    E\<^sub>G [simp]: "E\<^sub>G \<equiv> clause.to_ground (E \<cdot> \<rho>\<^sub>1 \<odot> \<gamma>)" and
+    D\<^sub>G [simp]: "D\<^sub>G \<equiv> clause.to_ground (D \<cdot> \<rho>\<^sub>2 \<odot> \<gamma>)" and
+    C\<^sub>G [simp]: "C\<^sub>G \<equiv> clause.to_ground (C \<cdot> \<gamma>)" and
+    N\<^sub>G [simp]: "N\<^sub>G \<equiv> clause_groundings (E, \<V>\<^sub>1) \<union> clause_groundings (D, \<V>\<^sub>2)" and
+    \<iota>\<^sub>G [simp]: "\<iota>\<^sub>G \<equiv> Infer [D\<^sub>G, E\<^sub>G] C\<^sub>G"
+  assumes
+    ground_superposition: "ground.superposition D\<^sub>G E\<^sub>G C\<^sub>G" and
+    \<rho>\<^sub>1: "term_subst.is_renaming \<rho>\<^sub>1" and
+    \<rho>\<^sub>2: "term_subst.is_renaming \<rho>\<^sub>2" and
+    rename_apart: "clause.vars (E \<cdot> \<rho>\<^sub>1) \<inter> clause.vars (D \<cdot> \<rho>\<^sub>2) = {}" and
+    E_grounding: "clause.is_ground (E \<cdot> \<rho>\<^sub>1 \<odot> \<gamma>)" and
+    D_grounding: "clause.is_ground (D \<cdot> \<rho>\<^sub>2 \<odot> \<gamma>)" and
+    C_grounding: "clause.is_ground (C \<cdot> \<gamma>)" and
+    select_from_E: "clause.from_ground (select\<^sub>G E\<^sub>G) = (select E) \<cdot> \<rho>\<^sub>1 \<odot> \<gamma>" and
+    select_from_D: "clause.from_ground (select\<^sub>G D\<^sub>G) = (select D) \<cdot> \<rho>\<^sub>2 \<odot> \<gamma>" and
+    E_is_welltyped: "clause.is_welltyped \<V>\<^sub>1 E" and
+    D_is_welltyped: "clause.is_welltyped \<V>\<^sub>2 D" and
+    \<rho>\<^sub>1_\<gamma>_is_welltyped: "is_welltyped_on (clause.vars E) \<V>\<^sub>1 (\<rho>\<^sub>1 \<odot> \<gamma>)" and
+    \<rho>\<^sub>2_\<gamma>_is_welltyped: "is_welltyped_on (clause.vars D) \<V>\<^sub>2 (\<rho>\<^sub>2 \<odot> \<gamma>)" and
+    \<rho>\<^sub>1_is_welltyped: "is_welltyped_on (clause.vars E) \<V>\<^sub>1 \<rho>\<^sub>1" and
+    \<rho>\<^sub>2_is_welltyped: "is_welltyped_on (clause.vars D) \<V>\<^sub>2 \<rho>\<^sub>2" and
+    \<V>\<^sub>1: "infinite_variables_per_type \<V>\<^sub>1" and
+    \<V>\<^sub>2: "infinite_variables_per_type \<V>\<^sub>2" and
+    non_redundant: "\<iota>\<^sub>G \<notin> ground.Red_I N\<^sub>G"
+  obtains C' \<V>\<^sub>3
   where
-    "superposition (premise\<^sub>2, \<V>\<^sub>2) (premise\<^sub>1, \<V>\<^sub>1) (conclusion', \<V>\<^sub>3)"
-    "\<iota>\<^sub>G \<in> inference_groundings (Infer [(premise\<^sub>2, \<V>\<^sub>2), (premise\<^sub>1, \<V>\<^sub>1)] (conclusion', \<V>\<^sub>3))"
-    "conclusion' \<cdot> \<gamma> = conclusion \<cdot> \<gamma>"
+    "superposition (D, \<V>\<^sub>2) (E, \<V>\<^sub>1) (C', \<V>\<^sub>3)"
+    "\<iota>\<^sub>G \<in> inference_groundings (Infer [(D, \<V>\<^sub>2), (E, \<V>\<^sub>1)] (C', \<V>\<^sub>3))"
+    "C' \<cdot> \<gamma> = C \<cdot> \<gamma>"
   using ground_superposition
-proof(cases premise\<^sub>G\<^sub>2 premise\<^sub>G\<^sub>1 conclusion\<^sub>G rule: ground.superposition.cases)
-  case ground_superpositionI: (superpositionI 
-      literal\<^sub>G\<^sub>1
-      premise\<^sub>G\<^sub>1'
-      literal\<^sub>G\<^sub>2
-      premise\<^sub>G\<^sub>2'
-      \<P>\<^sub>G
-      context\<^sub>G
-      term\<^sub>G\<^sub>1
-      term\<^sub>G\<^sub>2
-      term\<^sub>G\<^sub>3
-      )
+proof(cases D\<^sub>G E\<^sub>G C\<^sub>G rule: ground.superposition.cases)
+  case ground_superpositionI: (superpositionI l\<^sub>G\<^sub>1 E\<^sub>G' l\<^sub>G\<^sub>2 D\<^sub>G' \<P>\<^sub>G c\<^sub>G t\<^sub>G\<^sub>1 t\<^sub>G\<^sub>2 t\<^sub>G\<^sub>3)
 
-  have premise\<^sub>1_not_empty: "premise\<^sub>1 \<noteq> {#}"
-    using ground_superpositionI(1) empty_not_add_mset clause_subst_empty premise\<^sub>G\<^sub>1
-    by (metis clause_from_ground_empty_mset clause.from_ground_inverse)
+  have E_\<gamma>: "E \<cdot> \<rho>\<^sub>1 \<odot> \<gamma> = clause.from_ground (add_mset l\<^sub>G\<^sub>1 E\<^sub>G')"
+    using ground_superpositionI(1) E\<^sub>G
+    by (metis E_grounding clause.to_ground_inverse)
 
-  have premise\<^sub>2_not_empty: "premise\<^sub>2 \<noteq> {#}"
-    using ground_superpositionI(2) empty_not_add_mset clause_subst_empty premise\<^sub>G\<^sub>2
-    by (metis clause_from_ground_empty_mset clause.from_ground_inverse)
+  have D_\<gamma>: "D \<cdot> \<rho>\<^sub>2 \<odot> \<gamma> = clause.from_ground (add_mset l\<^sub>G\<^sub>2 D\<^sub>G')"
+    using ground_superpositionI(2) D\<^sub>G
+    by (metis D_grounding clause.to_ground_inverse)
 
-  have premise\<^sub>1_\<gamma>: "premise\<^sub>1 \<cdot> \<rho>\<^sub>1 \<cdot> \<gamma> = clause.from_ground (add_mset literal\<^sub>G\<^sub>1 premise\<^sub>G\<^sub>1')"
-    using ground_superpositionI(1) premise\<^sub>G\<^sub>1
-    by (metis premise\<^sub>1_grounding clause.to_ground_inverse)
+  let ?select\<^sub>G_empty = "select\<^sub>G (clause.to_ground (E \<cdot> \<rho>\<^sub>1 \<odot> \<gamma>)) = {#}"
+  let ?select\<^sub>G_not_empty = "select\<^sub>G (clause.to_ground (E \<cdot> \<rho>\<^sub>1 \<odot> \<gamma>)) \<noteq> {#}"
 
-  have premise\<^sub>2_\<gamma>: "premise\<^sub>2 \<cdot> \<rho>\<^sub>2 \<cdot> \<gamma> = clause.from_ground (add_mset literal\<^sub>G\<^sub>2 premise\<^sub>G\<^sub>2')"
-    using ground_superpositionI(2) premise\<^sub>G\<^sub>2
-    by (metis premise\<^sub>2_grounding clause.to_ground_inverse)
-
-  let ?select\<^sub>G_empty = "select\<^sub>G (clause.to_ground (premise\<^sub>1 \<cdot> \<rho>\<^sub>1 \<cdot> \<gamma>)) = {#}"
-  let ?select\<^sub>G_not_empty = "select\<^sub>G (clause.to_ground (premise\<^sub>1 \<cdot> \<rho>\<^sub>1 \<cdot> \<gamma>)) \<noteq> {#}"
-
-  have pos_literal\<^sub>G\<^sub>1_is_strictly_maximal\<^sub>l: 
-    "is_strictly_maximal (literal.from_ground literal\<^sub>G\<^sub>1) (premise\<^sub>1 \<cdot> \<rho>\<^sub>1 \<odot> \<gamma>)" if "\<P>\<^sub>G = Pos"
-    using ground_superpositionI(9) that
-    by(simp add: premise\<^sub>1_grounding)
-
-  have neg_literal\<^sub>G\<^sub>1_is_maximal\<^sub>l: 
-    "is_maximal (literal.from_ground literal\<^sub>G\<^sub>1) (premise\<^sub>1 \<cdot> \<rho>\<^sub>1 \<odot> \<gamma>)" if ?select\<^sub>G_empty
-    using
-      that
-      ground_superpositionI(9)  
-      is_maximal_if_is_strictly_maximal 
-      is_maximal_empty
-      premise\<^sub>1_\<gamma>
-    by auto
-
-  obtain pos_literal\<^sub>1 where
-    "is_strictly_maximal pos_literal\<^sub>1 premise\<^sub>1"
-    "pos_literal\<^sub>1 \<cdot>l \<rho>\<^sub>1 \<odot> \<gamma> = literal.from_ground literal\<^sub>G\<^sub>1" 
-  if "\<P>\<^sub>G = Pos"
-    using obtain_strictly_maximal_literal[OF 
-        premise\<^sub>1_grounding[folded clause.subst_comp_subst] 
-        pos_literal\<^sub>G\<^sub>1_is_strictly_maximal\<^sub>l
-        ]
-    by metis
-
-  moreover then have "pos_literal\<^sub>1 \<in># premise\<^sub>1" if "\<P>\<^sub>G = Pos"
-    using that strictly_maximal_in_clause by fastforce
-
-  moreover obtain neg_max_literal\<^sub>1 where
-    "is_maximal neg_max_literal\<^sub>1 premise\<^sub>1"
-    "neg_max_literal\<^sub>1 \<cdot>l \<rho>\<^sub>1 \<odot> \<gamma> = literal.from_ground literal\<^sub>G\<^sub>1" 
-  if "\<P>\<^sub>G = Neg" ?select\<^sub>G_empty
-    using 
-      obtain_maximal_literal[OF 
-        premise\<^sub>1_not_empty 
-        premise\<^sub>1_grounding[folded clause.subst_comp_subst]
-        ]
-      neg_literal\<^sub>G\<^sub>1_is_maximal\<^sub>l
-    by (metis (no_types, opaque_lifting) assms(9) clause.comp_subst.left.monoid_action_compatibility unique_maximal_in_ground_clause)
-
-  moreover then have "neg_max_literal\<^sub>1 \<in># premise\<^sub>1" if "\<P>\<^sub>G = Neg" ?select\<^sub>G_empty
-    using that maximal_in_clause by fastforce
-
-  moreover obtain neg_selected_literal\<^sub>1 where
-    "is_maximal neg_selected_literal\<^sub>1 (select premise\<^sub>1)"
-    "neg_selected_literal\<^sub>1 \<cdot>l \<rho>\<^sub>1 \<odot> \<gamma> = literal.from_ground literal\<^sub>G\<^sub>1" 
-  if "\<P>\<^sub>G = Neg" ?select\<^sub>G_not_empty 
+  obtain l\<^sub>1 where
+    l\<^sub>1_\<gamma>: "l\<^sub>1 \<cdot>l \<rho>\<^sub>1 \<odot> \<gamma> = literal.from_ground l\<^sub>G\<^sub>1" and
+    l\<^sub>1_is_strictly_maximal: "\<P>\<^sub>G = Pos \<Longrightarrow> is_strictly_maximal l\<^sub>1 E" and
+    l\<^sub>1_is_maximal: "\<P>\<^sub>G = Neg \<Longrightarrow> ?select\<^sub>G_empty \<Longrightarrow> is_maximal l\<^sub>1 E" and
+    l\<^sub>1_selected: "\<P>\<^sub>G = Neg \<Longrightarrow> ?select\<^sub>G_not_empty \<Longrightarrow> is_maximal l\<^sub>1 (select E)" and
+    l\<^sub>1_in_E: "l\<^sub>1 \<in># E"
   proof-
-    have "ground_is_maximal literal\<^sub>G\<^sub>1 (select\<^sub>G premise\<^sub>G\<^sub>1)" if "\<P>\<^sub>G = Neg" ?select\<^sub>G_not_empty
+
+    have E_not_empty: "E \<noteq> {#}"
+      using ground_superpositionI(1) 
+      by auto
+
+    have "is_strictly_maximal (literal.from_ground l\<^sub>G\<^sub>1) (E \<cdot> \<rho>\<^sub>1 \<odot> \<gamma>)" if "\<P>\<^sub>G = Pos"
+      using ground_superpositionI(9) that E_grounding
+      by simp
+
+    then obtain positive_l\<^sub>1 where
+      "is_strictly_maximal positive_l\<^sub>1 E"
+      "positive_l\<^sub>1 \<cdot>l \<rho>\<^sub>1 \<odot> \<gamma> = literal.from_ground l\<^sub>G\<^sub>1" 
+    if "\<P>\<^sub>G = Pos"
+      using obtain_strictly_maximal_literal[OF E_grounding]
+      by metis
+
+    moreover then have "positive_l\<^sub>1 \<in># E" if "\<P>\<^sub>G = Pos"
+      using that strictly_maximal_in_clause
+      by blast
+
+    moreover then have "is_maximal (literal.from_ground l\<^sub>G\<^sub>1) (E \<cdot> \<rho>\<^sub>1 \<odot> \<gamma>)" if ?select\<^sub>G_empty
+      using that ground_superpositionI(9) is_maximal_empty E_grounding
+      by auto
+
+    then obtain negative_maximal_l\<^sub>1 where
+      "is_maximal negative_maximal_l\<^sub>1 E"
+      "negative_maximal_l\<^sub>1 \<cdot>l \<rho>\<^sub>1 \<odot> \<gamma> = literal.from_ground l\<^sub>G\<^sub>1"
+    if "\<P>\<^sub>G = Neg" ?select\<^sub>G_empty
+      using
+        obtain_maximal_literal[OF E_not_empty E_grounding[folded clause.subst_comp_subst]]
+        unique_maximal_in_ground_clause[OF E_grounding[folded clause.subst_comp_subst]]
+      by metis
+
+    moreover then have "negative_maximal_l\<^sub>1 \<in># E" if "\<P>\<^sub>G = Neg" ?select\<^sub>G_empty
+      using that maximal_in_clause
+      by blast
+
+    moreover have "ground_is_maximal l\<^sub>G\<^sub>1 (select\<^sub>G E\<^sub>G)" if "\<P>\<^sub>G = Neg" ?select\<^sub>G_not_empty
       using ground_superpositionI(9) that
       by simp
 
-    then show ?thesis
-      using
-        that 
-        select(1) 
+    then obtain negative_selected_l\<^sub>1 where
+      "is_maximal negative_selected_l\<^sub>1 (select E)"
+      "negative_selected_l\<^sub>1 \<cdot>l \<rho>\<^sub>1 \<odot> \<gamma> = literal.from_ground l\<^sub>G\<^sub>1" 
+    if "\<P>\<^sub>G = Neg" ?select\<^sub>G_not_empty
+      using 
+        select_from_E
         unique_maximal_in_ground_clause
         obtain_maximal_literal
-      unfolding premise\<^sub>G\<^sub>1
-      by (metis (mono_tags, lifting) clause.comp_subst.monoid_action_compatibility 
-          clause_subst_empty(2) clause.ground_is_ground image_mset_is_empty_iff 
-          clause.from_ground_def)
+      unfolding E\<^sub>G
+      by (metis (no_types, lifting) clause.ground_is_ground clause_from_ground_empty 
+          clause_subst_empty)
+
+    moreover then have "negative_selected_l\<^sub>1 \<in># E" if "\<P>\<^sub>G = Neg" ?select\<^sub>G_not_empty 
+      using that
+      by (meson maximal_in_clause mset_subset_eqD select_subset)
+
+    ultimately show ?thesis
+      using that ground_superpositionI(9)
+      by (metis literals_distinct(1))
   qed
 
-  moreover then have "neg_selected_literal\<^sub>1 \<in># premise\<^sub>1" if "\<P>\<^sub>G = Neg" ?select\<^sub>G_not_empty 
-    using that
-    by (meson maximal_in_clause mset_subset_eqD select_subset)
+  obtain E' where E: "E = add_mset l\<^sub>1 E'"
+    by (meson l\<^sub>1_in_E multi_member_split)
 
-  ultimately obtain literal\<^sub>1 where
-    literal\<^sub>1_\<gamma>: "literal\<^sub>1 \<cdot>l \<rho>\<^sub>1 \<odot> \<gamma> = literal.from_ground literal\<^sub>G\<^sub>1" and
-    literal\<^sub>1_in_premise\<^sub>1: "literal\<^sub>1 \<in># premise\<^sub>1" and
-    literal\<^sub>1_is_strictly_maximal: "\<P>\<^sub>G = Pos \<Longrightarrow> is_strictly_maximal literal\<^sub>1 premise\<^sub>1" and
-    literal\<^sub>1_is_maximal: "\<P>\<^sub>G = Neg \<Longrightarrow> ?select\<^sub>G_empty \<Longrightarrow> is_maximal literal\<^sub>1 premise\<^sub>1" and
-    literal\<^sub>1_selected: "\<P>\<^sub>G = Neg \<Longrightarrow> ?select\<^sub>G_not_empty \<Longrightarrow> is_maximal literal\<^sub>1 (select premise\<^sub>1)"
-    by (metis ground_superpositionI(9) literals_distinct(1))
-
-  then have literal\<^sub>1_grounding: "literal.is_ground (literal\<^sub>1 \<cdot>l \<rho>\<^sub>1 \<odot> \<gamma>)"
-    by simp
-
-  have literal\<^sub>G\<^sub>2_is_strictly_maximal\<^sub>l: 
-    "is_strictly_maximal (literal.from_ground literal\<^sub>G\<^sub>2) (premise\<^sub>2 \<cdot> \<rho>\<^sub>2 \<odot> \<gamma>)"
-    using ground_superpositionI(11)
-    by (simp add: premise\<^sub>2_grounding)
-
-  obtain literal\<^sub>2 where 
-    literal\<^sub>2_strictly_maximal: "is_strictly_maximal literal\<^sub>2 premise\<^sub>2" and
-    literal\<^sub>2_\<gamma>: "literal\<^sub>2 \<cdot>l \<rho>\<^sub>2 \<odot> \<gamma> = literal.from_ground literal\<^sub>G\<^sub>2"
-    using obtain_strictly_maximal_literal[OF 
-        premise\<^sub>2_grounding[folded clause.subst_comp_subst] 
-        literal\<^sub>G\<^sub>2_is_strictly_maximal\<^sub>l
-        ]
-    by metis
-
-  then have literal\<^sub>2_in_premise\<^sub>2: "literal\<^sub>2 \<in># premise\<^sub>2" 
-    using strictly_maximal_in_clause by blast
-
-  have literal\<^sub>2_grounding: "literal.is_ground (literal\<^sub>2 \<cdot>l \<rho>\<^sub>2 \<odot> \<gamma>)"
-    using literal\<^sub>2_\<gamma> by simp
-
-  obtain premise\<^sub>1' where premise\<^sub>1: "premise\<^sub>1 = add_mset literal\<^sub>1 premise\<^sub>1'"
-    by (meson literal\<^sub>1_in_premise\<^sub>1 multi_member_split)
-
-  then have premise\<^sub>1'_\<gamma>: "premise\<^sub>1' \<cdot> \<rho>\<^sub>1 \<cdot> \<gamma> = clause.from_ground premise\<^sub>G\<^sub>1'"
-    using premise\<^sub>1_\<gamma>  
-    unfolding clause.from_ground_add  literal\<^sub>1_\<gamma>[symmetric]
-    by simp
-
-  obtain premise\<^sub>2' where premise\<^sub>2: "premise\<^sub>2 = add_mset literal\<^sub>2 premise\<^sub>2'"
-    by (meson literal\<^sub>2_in_premise\<^sub>2 multi_member_split)
-
-  then have premise\<^sub>2'_\<gamma>: "premise\<^sub>2' \<cdot> \<rho>\<^sub>2 \<cdot> \<gamma> = clause.from_ground premise\<^sub>G\<^sub>2'"
-    using premise\<^sub>2_\<gamma>  
-    unfolding clause.from_ground_add literal\<^sub>2_\<gamma>[symmetric]
-    by simp
+  then have E'_\<gamma>: "E' \<cdot> \<rho>\<^sub>1 \<odot> \<gamma> = clause.from_ground E\<^sub>G'"
+    using l\<^sub>1_\<gamma> E_\<gamma>
+    by auto
 
   let ?\<P> = "if \<P>\<^sub>G = Pos then Pos else Neg"
 
-  have [simp]: "\<P>\<^sub>G \<noteq> Pos \<longleftrightarrow> \<P>\<^sub>G = Neg"
-    using ground_superpositionI(4) 
+  have [simp]: "\<P>\<^sub>G \<noteq> Pos \<longleftrightarrow> \<P>\<^sub>G = Neg" "\<P>\<^sub>G \<noteq> Neg \<longleftrightarrow> \<P>\<^sub>G = Pos"
+    using ground_superpositionI(4)
     by auto
 
-  have "literal\<^sub>1 \<cdot>l \<rho>\<^sub>1 \<cdot>l \<gamma> = 
-    ?\<P> (Upair (context.from_ground context\<^sub>G)\<langle>term.from_ground term\<^sub>G\<^sub>1\<rangle> (term.from_ground term\<^sub>G\<^sub>2))"
-    using literal\<^sub>1_\<gamma>
-    unfolding ground_superpositionI(5)
+  have [simp]: "\<And>a \<sigma>. ?\<P> a \<cdot>l \<sigma> = ?\<P> (a \<cdot>a \<sigma>)"
+    by auto
+
+  have [simp]: "\<And>\<V> a. literal.is_welltyped \<V> (?\<P> a) \<longleftrightarrow> atom.is_welltyped \<V> a"
+    by(auto simp: literal_is_welltyped_iff_atm_of)
+
+  have [simp]: "\<And>a. literal.vars (?\<P> a) = atom.vars a"
+    by auto
+
+  have l\<^sub>1_\<gamma>: 
+    "l\<^sub>1 \<cdot>l \<rho>\<^sub>1 \<odot> \<gamma> = ?\<P> (Upair (context.from_ground c\<^sub>G)\<langle>term.from_ground t\<^sub>G\<^sub>1\<rangle> (term.from_ground t\<^sub>G\<^sub>2))"
+    unfolding ground_superpositionI l\<^sub>1_\<gamma>
     by simp
 
-  then obtain term\<^sub>1_with_context term\<^sub>1' where 
-    literal\<^sub>1: "literal\<^sub>1 = ?\<P> (Upair term\<^sub>1_with_context term\<^sub>1')" and
-    term\<^sub>1'_\<gamma>: "term\<^sub>1' \<cdot>t \<rho>\<^sub>1 \<cdot>t \<gamma> = term.from_ground term\<^sub>G\<^sub>2" and
-    term\<^sub>1_with_context_\<gamma>: 
-      "term\<^sub>1_with_context \<cdot>t \<rho>\<^sub>1 \<cdot>t \<gamma> = (context.from_ground context\<^sub>G)\<langle>term.from_ground term\<^sub>G\<^sub>1\<rangle>"
-    by (smt (verit) obtain_from_literal_subst)
-
-  from literal\<^sub>2_\<gamma> have "literal\<^sub>2 \<cdot>l \<rho>\<^sub>2 \<cdot>l \<gamma> = term.from_ground term\<^sub>G\<^sub>1 \<approx> term.from_ground term\<^sub>G\<^sub>3"
-    unfolding ground_superpositionI(6) atom_from_ground_term_from_ground 
-      literal_from_ground_atom_from_ground(2) literal.subst_comp_subst.
-
-  then obtain term\<^sub>2 term\<^sub>2' where 
-    literal\<^sub>2: "literal\<^sub>2 = term\<^sub>2 \<approx> term\<^sub>2'" and
-    term\<^sub>2_\<gamma>: "term\<^sub>2 \<cdot>t \<rho>\<^sub>2 \<cdot>t \<gamma> = term.from_ground term\<^sub>G\<^sub>1" and     
-    term\<^sub>2'_\<gamma>: "term\<^sub>2' \<cdot>t \<rho>\<^sub>2 \<cdot>t \<gamma> = term.from_ground term\<^sub>G\<^sub>3"
-    using obtain_from_pos_literal_subst
-    by metis
-
-  let ?inference_into_var = "\<nexists>context\<^sub>1 term\<^sub>1. 
-      term\<^sub>1_with_context = context\<^sub>1\<langle>term\<^sub>1\<rangle> \<and> 
-      term\<^sub>1 \<cdot>t \<rho>\<^sub>1 \<cdot>t \<gamma> = term.from_ground term\<^sub>G\<^sub>1 \<and> 
-      context\<^sub>1 \<cdot>t\<^sub>c \<rho>\<^sub>1 \<cdot>t\<^sub>c \<gamma> = context.from_ground context\<^sub>G \<and> 
-      is_Fun term\<^sub>1"
-
-  have inference_into_var_is_redundant: 
-    "?inference_into_var \<Longrightarrow> ground.redundant_infer premise_groundings \<iota>\<^sub>G"
+  obtain c\<^sub>1 t\<^sub>1 t\<^sub>1' where 
+    l\<^sub>1: "l\<^sub>1 = ?\<P> (Upair c\<^sub>1\<langle>t\<^sub>1\<rangle> t\<^sub>1')" and
+    t\<^sub>1'_\<gamma>: "t\<^sub>1' \<cdot>t \<rho>\<^sub>1 \<odot> \<gamma> = term.from_ground t\<^sub>G\<^sub>2" and
+    t\<^sub>1_\<gamma>: "t\<^sub>1 \<cdot>t \<rho>\<^sub>1 \<odot> \<gamma> = term.from_ground t\<^sub>G\<^sub>1" and
+    c\<^sub>1_\<gamma>: "c\<^sub>1 \<cdot>t\<^sub>c \<rho>\<^sub>1 \<odot> \<gamma> = context.from_ground c\<^sub>G" and
+    t\<^sub>1_is_Fun: "is_Fun t\<^sub>1"
   proof-
-    assume inference_into_var: ?inference_into_var
 
-    obtain term\<^sub>x context\<^sub>x context\<^sub>x' where
-      term\<^sub>1_with_context: "term\<^sub>1_with_context = context\<^sub>x\<langle>term\<^sub>x\<rangle>" and
-      is_Var_term\<^sub>x: "is_Var term\<^sub>x" and
-      "context.from_ground context\<^sub>G = (context\<^sub>x \<cdot>t\<^sub>c \<rho>\<^sub>1 \<cdot>t\<^sub>c \<gamma>) \<circ>\<^sub>c context\<^sub>x'"
-    proof-  
-      from inference_into_var term\<^sub>1_with_context_\<gamma>
-      have 
-        "\<exists>term\<^sub>x context\<^sub>x context\<^sub>x'. 
-        term\<^sub>1_with_context = context\<^sub>x\<langle>term\<^sub>x\<rangle> \<and> 
-        is_Var term\<^sub>x \<and> 
-        context.from_ground context\<^sub>G = (context\<^sub>x \<cdot>t\<^sub>c \<rho>\<^sub>1 \<cdot>t\<^sub>c \<gamma>) \<circ>\<^sub>c context\<^sub>x'"
-      proof(induction term\<^sub>1_with_context arbitrary: context\<^sub>G)
+    obtain c\<^sub>1_t\<^sub>1 t\<^sub>1' where 
+      l\<^sub>1: "l\<^sub>1 = ?\<P> (Upair c\<^sub>1_t\<^sub>1 t\<^sub>1')" and
+      t\<^sub>1'_\<gamma>: "t\<^sub>1' \<cdot>t \<rho>\<^sub>1 \<odot> \<gamma> = term.from_ground t\<^sub>G\<^sub>2" and
+      c\<^sub>1_t\<^sub>1_\<gamma>: "c\<^sub>1_t\<^sub>1 \<cdot>t \<rho>\<^sub>1 \<odot> \<gamma> = (context.from_ground c\<^sub>G)\<langle>term.from_ground t\<^sub>G\<^sub>1\<rangle>"
+      using l\<^sub>1_\<gamma>
+      by (smt (verit) obtain_from_literal_subst)
+
+    let ?inference_into_Fun =
+      "\<exists>c\<^sub>1 t\<^sub>1. 
+        c\<^sub>1_t\<^sub>1 = c\<^sub>1\<langle>t\<^sub>1\<rangle> \<and>
+        t\<^sub>1 \<cdot>t \<rho>\<^sub>1 \<odot> \<gamma> = term.from_ground t\<^sub>G\<^sub>1 \<and>
+        c\<^sub>1 \<cdot>t\<^sub>c \<rho>\<^sub>1 \<odot> \<gamma> = context.from_ground c\<^sub>G \<and>
+        is_Fun t\<^sub>1"
+
+    have "\<not> ?inference_into_Fun \<Longrightarrow> ground.redundant_infer N\<^sub>G \<iota>\<^sub>G"
+    proof-
+      assume "\<not> ?inference_into_Fun"
+
+      with c\<^sub>1_t\<^sub>1_\<gamma>
+      obtain t\<^sub>1 c\<^sub>1 c\<^sub>G' where
+        c\<^sub>1_t\<^sub>1: "c\<^sub>1_t\<^sub>1 = c\<^sub>1\<langle>t\<^sub>1\<rangle>" and
+        t\<^sub>1_is_Var: "is_Var t\<^sub>1" and
+        c\<^sub>G: "c\<^sub>G = context.to_ground (c\<^sub>1 \<cdot>t\<^sub>c \<rho>\<^sub>1 \<odot> \<gamma>) \<circ>\<^sub>c c\<^sub>G'"
+      proof(induction c\<^sub>1_t\<^sub>1 arbitrary: c\<^sub>G thesis)
         case (Var x)
+
         show ?case
-        proof(intro exI conjI)
-          show
-            "Var x = \<box>\<langle>Var x\<rangle>"
-            "is_Var (Var x)"
-            "context.from_ground context\<^sub>G = (\<box> \<cdot>t\<^sub>c \<rho>\<^sub>1 \<cdot>t\<^sub>c \<gamma>) \<circ>\<^sub>c context.from_ground context\<^sub>G"
-            by simp_all
+        proof(rule Var.prems)
+          show "Var x = \<box>\<langle>Var x\<rangle>"
+            by simp
+
+          show "is_Var (Var x)"
+            by simp
+
+          show "c\<^sub>G = context.to_ground (\<box> \<cdot>t\<^sub>c \<rho>\<^sub>1 \<odot> \<gamma>) \<circ>\<^sub>c c\<^sub>G"
+            by (simp add: context.to_ground_def)
         qed
       next
-        case (Fun f terms)
+        case (Fun f ts)
 
-        then have "context\<^sub>G \<noteq> Hole"
-          by (metis Fun.prems(2) actxt.simps(8) context.context_from_ground_hole intp_actxt.simps(1) 
-              is_FunI)
-
-        then obtain terms\<^sub>G\<^sub>1 context\<^sub>G' terms\<^sub>G\<^sub>2 where
-          context\<^sub>G: "context\<^sub>G = More f terms\<^sub>G\<^sub>1 context\<^sub>G' terms\<^sub>G\<^sub>2"
-          using Fun(3)
-          by(cases context\<^sub>G)(auto simp: context.from_ground_def)
-
-        have terms_\<gamma>: 
-          "map (\<lambda>term. term \<cdot>t \<rho>\<^sub>1 \<cdot>t \<gamma>) terms = 
-            map term.from_ground terms\<^sub>G\<^sub>1 @ (context.from_ground context\<^sub>G')\<langle>term.from_ground term\<^sub>G\<^sub>1\<rangle> #
-             map term.from_ground terms\<^sub>G\<^sub>2"
-          using Fun(3) 
-          unfolding context\<^sub>G context.from_ground_def
-          (* TODO *)
-          by (smt (verit, best) actxt.simps(9) eval_subst eval_term.simps(2) intp_actxt.simps(2) map_eq_conv term.inject(2))
-        
-        then obtain terms\<^sub>1 "term" terms\<^sub>2 where 
-          terms: "terms = terms\<^sub>1 @ term # terms\<^sub>2" and
-          terms\<^sub>1_\<gamma>: "map (\<lambda>term. term \<cdot>t \<rho>\<^sub>1 \<cdot>t \<gamma>) terms\<^sub>1 = map term.from_ground terms\<^sub>G\<^sub>1" and
-          terms\<^sub>2_\<gamma>: "map (\<lambda>term. term \<cdot>t \<rho>\<^sub>1 \<cdot>t \<gamma>) terms\<^sub>2 = map term.from_ground terms\<^sub>G\<^sub>2"  
+        have "c\<^sub>G \<noteq> \<box>"
+          using Fun.prems(2,3)
           unfolding context.from_ground_def
-          (* TODO *)
-          by (smt (z3) append_eq_map_conv map_eq_Cons_D)
+          by (metis actxt.simps(8) intp_actxt.simps(1) is_FunI)
 
-        with terms_\<gamma> 
-        have term_\<gamma>: "term \<cdot>t \<rho>\<^sub>1 \<cdot>t \<gamma> = (context.from_ground context\<^sub>G')\<langle>term.from_ground term\<^sub>G\<^sub>1\<rangle>"
+        then obtain ts\<^sub>G\<^sub>1 c\<^sub>G' ts\<^sub>G\<^sub>2 where
+          c\<^sub>G: "c\<^sub>G = More f ts\<^sub>G\<^sub>1 c\<^sub>G' ts\<^sub>G\<^sub>2"
+          using Fun.prems
+          by (cases c\<^sub>G) (auto simp: context.from_ground_def)
+
+        have
+          "map (\<lambda>t. t \<cdot>t \<rho>\<^sub>1 \<odot> \<gamma>) ts =
+            map term.from_ground ts\<^sub>G\<^sub>1 @ (context.from_ground c\<^sub>G')\<langle>term.from_ground t\<^sub>G\<^sub>1\<rangle> # 
+            map term.from_ground ts\<^sub>G\<^sub>2"
+          using Fun(3)
+          unfolding c\<^sub>G context.from_ground_def
           by simp
 
-        show ?case
-        proof(cases "term.is_ground term")
-          case True
+        moreover then obtain ts\<^sub>1 t ts\<^sub>2 where 
+          ts: "ts = ts\<^sub>1 @ t # ts\<^sub>2" and
+          ts\<^sub>1_\<gamma>: "map (\<lambda>term. term \<cdot>t \<rho>\<^sub>1 \<odot> \<gamma>) ts\<^sub>1 = map term.from_ground ts\<^sub>G\<^sub>1" and
+          ts\<^sub>2_\<gamma>: "map (\<lambda>term. term \<cdot>t \<rho>\<^sub>1 \<odot> \<gamma>) ts\<^sub>2 = map term.from_ground ts\<^sub>G\<^sub>2"            
+          by (smt append_eq_map_conv map_eq_Cons_D)
 
-          with term_\<gamma> 
-          obtain term\<^sub>1 context\<^sub>1 where
-            "term = context\<^sub>1\<langle>term\<^sub>1\<rangle>"
-            "term\<^sub>1 \<cdot>t \<rho>\<^sub>1 \<cdot>t \<gamma> = term.from_ground term\<^sub>G\<^sub>1" 
-            "context\<^sub>1 \<cdot>t\<^sub>c \<rho>\<^sub>1 \<cdot>t\<^sub>c \<gamma> = context.from_ground context\<^sub>G'" 
-            "is_Fun term\<^sub>1"
-            by (metis Term.ground_vars_term_empty context.ground_is_ground ground_subst_apply 
-                term.ground_is_ground context.subst_ident_if_ground gterm_is_fun)
+        ultimately have t_\<gamma>: "t \<cdot>t \<rho>\<^sub>1 \<odot> \<gamma> = (context.from_ground c\<^sub>G')\<langle>term.from_ground t\<^sub>G\<^sub>1\<rangle>"
+          by simp
 
-          moreover then have "Fun f terms = (More f terms\<^sub>1 context\<^sub>1 terms\<^sub>2)\<langle>term\<^sub>1\<rangle>"
-            unfolding terms
-            by auto
+        obtain t\<^sub>1 c\<^sub>1 c\<^sub>G'' where 
+          "t = c\<^sub>1\<langle>t\<^sub>1\<rangle>" and
+          "is_Var t\<^sub>1" and
+          "c\<^sub>G' = context.to_ground (c\<^sub>1 \<cdot>t\<^sub>c \<rho>\<^sub>1 \<odot> \<gamma>) \<circ>\<^sub>c c\<^sub>G''"
+        proof-
+          have "t \<in> set ts"
+            by (simp add: ts)
 
-          ultimately have 
-            "\<exists>context\<^sub>1 term\<^sub>1. 
-            Fun f terms = context\<^sub>1\<langle>term\<^sub>1\<rangle> \<and> 
-            term\<^sub>1 \<cdot>t \<rho>\<^sub>1 \<cdot>t \<gamma> = term.from_ground term\<^sub>G\<^sub>1 \<and> 
-            context\<^sub>1 \<cdot>t\<^sub>c \<rho>\<^sub>1 \<cdot>t\<^sub>c \<gamma> = context.from_ground context\<^sub>G \<and> 
-            is_Fun term\<^sub>1"
-             unfolding context.from_ground_def
-             by (auto
-                intro: exI[of _ "More f terms\<^sub>1 context\<^sub>1 terms\<^sub>2"] exI[of _ term\<^sub>1] 
-                simp: comp_def terms\<^sub>1_\<gamma> terms\<^sub>2_\<gamma> context\<^sub>G)
-            
-          then show ?thesis
-            using Fun(2)
-            by argo
-        next
-          case False
-          moreover have "term \<in> set terms"
-            using terms by auto
-
-          moreover have 
-            "\<nexists>context\<^sub>1 term\<^sub>1. term = context\<^sub>1\<langle>term\<^sub>1\<rangle> \<and> 
-            term\<^sub>1 \<cdot>t \<rho>\<^sub>1 \<cdot>t \<gamma> = term.from_ground term\<^sub>G\<^sub>1 \<and> 
-            context\<^sub>1 \<cdot>t\<^sub>c \<rho>\<^sub>1 \<cdot>t\<^sub>c \<gamma> = context.from_ground context\<^sub>G' \<and> 
-            is_Fun term\<^sub>1"
-          proof(rule notI)
+          moreover have
+            "\<nexists>c\<^sub>1 t\<^sub>1. t = c\<^sub>1\<langle>t\<^sub>1\<rangle> \<and> 
+                t\<^sub>1 \<cdot>t \<rho>\<^sub>1 \<odot> \<gamma> = term.from_ground t\<^sub>G\<^sub>1 \<and> 
+                c\<^sub>1 \<cdot>t\<^sub>c \<rho>\<^sub>1 \<odot> \<gamma> = context.from_ground c\<^sub>G' \<and> 
+                is_Fun t\<^sub>1"
+          proof(rule notI, elim exE conjE)
+            fix c\<^sub>1 t\<^sub>1
             assume 
-              "\<exists>context\<^sub>1 term\<^sub>1. 
-              term = context\<^sub>1\<langle>term\<^sub>1\<rangle> \<and> 
-              term\<^sub>1 \<cdot>t \<rho>\<^sub>1 \<cdot>t \<gamma> = term.from_ground term\<^sub>G\<^sub>1 \<and> 
-              context\<^sub>1 \<cdot>t\<^sub>c \<rho>\<^sub>1 \<cdot>t\<^sub>c \<gamma> = context.from_ground context\<^sub>G' \<and> 
-              is_Fun term\<^sub>1"
+              "t = c\<^sub>1\<langle>t\<^sub>1\<rangle>" 
+              "t\<^sub>1 \<cdot>t \<rho>\<^sub>1 \<odot> \<gamma> = term.from_ground t\<^sub>G\<^sub>1" 
+              "c\<^sub>1 \<cdot>t\<^sub>c \<rho>\<^sub>1 \<odot> \<gamma> = context.from_ground c\<^sub>G'" 
+              "is_Fun t\<^sub>1"
 
-            then obtain context\<^sub>1 term\<^sub>1 where
-              "term": "term = context\<^sub>1\<langle>term\<^sub>1\<rangle>"
-              "term\<^sub>1 \<cdot>t \<rho>\<^sub>1 \<cdot>t \<gamma> = term.from_ground term\<^sub>G\<^sub>1"
-              "context\<^sub>1 \<cdot>t\<^sub>c \<rho>\<^sub>1 \<cdot>t\<^sub>c \<gamma> = context.from_ground context\<^sub>G'"
-              "is_Fun term\<^sub>1"
+            moreover then have 
+              "Fun f ts = (More f ts\<^sub>1 c\<^sub>1 ts\<^sub>2)\<langle>t\<^sub>1\<rangle>" 
+              "(More f ts\<^sub>1 c\<^sub>1 ts\<^sub>2) \<cdot>t\<^sub>c \<rho>\<^sub>1 \<odot> \<gamma> = context.from_ground c\<^sub>G"
+              unfolding context.from_ground_def c\<^sub>G ts
+              using ts\<^sub>1_\<gamma> ts\<^sub>2_\<gamma>
+              by auto
+
+            ultimately show False
+              using Fun.prems(3)
               by blast
-
-            then have 
-              "\<exists>context\<^sub>1 term\<^sub>1. 
-              Fun f terms = context\<^sub>1\<langle>term\<^sub>1\<rangle> \<and> 
-              term\<^sub>1 \<cdot>t \<rho>\<^sub>1 \<cdot>t \<gamma> = term.from_ground term\<^sub>G\<^sub>1 \<and> 
-              context\<^sub>1 \<cdot>t\<^sub>c \<rho>\<^sub>1 \<cdot>t\<^sub>c \<gamma> = context.from_ground context\<^sub>G \<and> 
-              is_Fun term\<^sub>1"
-              unfolding context.from_ground_def
-              by(auto 
-                  intro: exI[of _ "(More f terms\<^sub>1 context\<^sub>1 terms\<^sub>2)"] exI[of _ term\<^sub>1] 
-                  simp: "term" terms terms\<^sub>1_\<gamma> terms\<^sub>2_\<gamma> context\<^sub>G comp_def)
-
-            then show False
-              using Fun(2)
-              by argo
           qed
 
-          ultimately obtain term\<^sub>x context\<^sub>x context\<^sub>x' where
-            "term = context\<^sub>x\<langle>term\<^sub>x\<rangle>"  
-            "is_Var term\<^sub>x" 
-            "context.from_ground context\<^sub>G' = (context\<^sub>x \<cdot>t\<^sub>c \<rho>\<^sub>1 \<cdot>t\<^sub>c \<gamma>) \<circ>\<^sub>c context\<^sub>x'"
-            using Fun(1) term_\<gamma> by blast
+          ultimately show ?thesis
+            using Fun(1) t_\<gamma> that
+            by blast
+        qed
 
-          then have 
-            "Fun f terms = (More f terms\<^sub>1 context\<^sub>x terms\<^sub>2)\<langle>term\<^sub>x\<rangle>"
-            "is_Var term\<^sub>x" 
-            "context.from_ground context\<^sub>G = (More f terms\<^sub>1 context\<^sub>x terms\<^sub>2 \<cdot>t\<^sub>c \<rho>\<^sub>1 \<cdot>t\<^sub>c \<gamma>) \<circ>\<^sub>c context\<^sub>x'"
-            unfolding context.from_ground_def
-            by(auto simp: terms terms\<^sub>1_\<gamma> terms\<^sub>2_\<gamma> context\<^sub>G comp_def)
+        moreover then have
+          "Fun f ts = (More f ts\<^sub>1 c\<^sub>1 ts\<^sub>2)\<langle>t\<^sub>1\<rangle>"
+          "c\<^sub>G = context.to_ground (More f ts\<^sub>1 c\<^sub>1 ts\<^sub>2 \<cdot>t\<^sub>c \<rho>\<^sub>1 \<odot> \<gamma>) \<circ>\<^sub>c c\<^sub>G''"
+          using ts\<^sub>1_\<gamma> ts\<^sub>2_\<gamma>
+          unfolding context.to_ground_def c\<^sub>G ts
+          by auto
+
+        ultimately show ?case
+          using Fun.prems(1)
+          by blast
+      qed
+
+      obtain x where t\<^sub>1_\<rho>\<^sub>1: "t\<^sub>1 \<cdot>t \<rho>\<^sub>1 = Var x"
+        using t\<^sub>1_is_Var term.id_subst_rename[OF \<rho>\<^sub>1]
+        unfolding is_Var_def
+        by auto
+
+      have \<iota>\<^sub>G_parts: 
+        "set (side_prems_of \<iota>\<^sub>G) = {D\<^sub>G}" 
+        "main_prem_of \<iota>\<^sub>G = E\<^sub>G"
+        "concl_of \<iota>\<^sub>G = C\<^sub>G"
+        unfolding \<iota>\<^sub>G
+        by simp_all
+
+      show ?thesis
+      proof(unfold ground.redundant_infer_def \<iota>\<^sub>G_parts, intro exI conjI)
+
+        let ?t\<^sub>G = "(context.from_ground c\<^sub>G')\<langle>term.from_ground t\<^sub>G\<^sub>3\<rangle>"
+
+        define \<gamma>' where
+          "\<gamma>' \<equiv> \<gamma>(x := ?t\<^sub>G)"
+
+        let ?E\<^sub>G' = "clause.to_ground (E \<cdot> \<rho>\<^sub>1 \<odot> \<gamma>')"
+
+        have t\<^sub>1_\<gamma>: "t\<^sub>1 \<cdot>t \<rho>\<^sub>1 \<odot> \<gamma> = (context.from_ground c\<^sub>G')\<langle>term.from_ground t\<^sub>G\<^sub>1\<rangle>"
+        proof -
+
+          have "context.is_ground (c\<^sub>1 \<cdot>t\<^sub>c \<rho>\<^sub>1 \<odot> \<gamma>)"
+            using c\<^sub>1_t\<^sub>1_\<gamma>
+            unfolding c\<^sub>1_t\<^sub>1 context.safe_unfolds
+            by (metis context.ground_is_ground context.term_with_context_is_ground 
+                term.ground_is_ground)
+
+          then show ?thesis
+            using c\<^sub>1_t\<^sub>1_\<gamma>
+            unfolding c\<^sub>1_t\<^sub>1 c\<^sub>1_t\<^sub>1_\<gamma> c\<^sub>G
+            by auto
+        qed
+
+        have t\<^sub>1_\<gamma>': "t\<^sub>1 \<cdot>t \<rho>\<^sub>1 \<odot> \<gamma>' = (context.from_ground c\<^sub>G')\<langle>term.from_ground t\<^sub>G\<^sub>3\<rangle>"
+          unfolding \<gamma>'_def
+          using t\<^sub>1_\<rho>\<^sub>1
+          by simp
+         
+        show "{?E\<^sub>G'} \<subseteq> N\<^sub>G"
+        proof-
+
+          have "?E\<^sub>G' \<in> clause_groundings (E, \<V>\<^sub>1)"
+          proof(unfold clause_groundings_def mem_Collect_eq fst_conv snd_conv, 
+              intro exI conjI E_is_welltyped \<V>\<^sub>1, 
+              rule refl)
+
+            show "clause.is_ground (E \<cdot> \<rho>\<^sub>1 \<odot> \<gamma>')"
+              unfolding \<gamma>'_def
+              using E_grounding
+              by simp
+
+            show "is_welltyped_on (clause.vars E) \<V>\<^sub>1 (\<rho>\<^sub>1 \<odot> \<gamma>')"
+            proof(intro is_welltyped_on_subst_compose \<rho>\<^sub>1_is_welltyped)
+              
+              have "welltyped \<V>\<^sub>1 ?t\<^sub>G (\<V>\<^sub>1 x)"
+              proof-
+
+                have "welltyped \<V>\<^sub>1 (context.from_ground c\<^sub>G')\<langle>term.from_ground t\<^sub>G\<^sub>1\<rangle> (\<V>\<^sub>1 x)"
+                proof-
+
+                  have "welltyped \<V>\<^sub>1 (t\<^sub>1 \<cdot>t \<rho>\<^sub>1) (\<V>\<^sub>1 x)"
+                    using t\<^sub>1_\<rho>\<^sub>1
+                    by auto
+
+                  then have "welltyped \<V>\<^sub>1 (t\<^sub>1 \<cdot>t \<rho>\<^sub>1 \<odot> \<gamma>) (\<V>\<^sub>1 x)"
+                    using \<rho>\<^sub>1_is_welltyped \<rho>\<^sub>1_\<gamma>_is_welltyped
+                    unfolding E c\<^sub>1_t\<^sub>1 l\<^sub>1 subst_compose_def
+                    by simp
+
+                  moreover have "context.is_ground (c\<^sub>1 \<cdot>t\<^sub>c \<rho>\<^sub>1 \<odot> \<gamma>)"
+                    using c\<^sub>1_t\<^sub>1_\<gamma> 
+                    unfolding c\<^sub>1_t\<^sub>1 context.safe_unfolds
+                    by (metis context.ground_is_ground context.term_with_context_is_ground 
+                        term.ground_is_ground)
+
+                  then have "t\<^sub>1 \<cdot>t \<rho>\<^sub>1 \<odot> \<gamma> = (context.from_ground c\<^sub>G')\<langle>term.from_ground t\<^sub>G\<^sub>1\<rangle>"
+                    using c\<^sub>1_t\<^sub>1_\<gamma>
+                    unfolding c\<^sub>1_t\<^sub>1 c\<^sub>1_t\<^sub>1_\<gamma> c\<^sub>G
+                    by auto
+
+                  ultimately show ?thesis
+                    by argo
+                qed
+
+                moreover obtain \<tau> where
+                  "welltyped \<V>\<^sub>1 (term.from_ground t\<^sub>G\<^sub>1) \<tau>" 
+                  "welltyped \<V>\<^sub>1 (term.from_ground t\<^sub>G\<^sub>3) \<tau>"
+                proof-
+                  have "clause.is_welltyped \<V>\<^sub>2 (clause.from_ground D\<^sub>G)"
+                    using D_is_welltyped
+                    unfolding
+                      D\<^sub>G
+                      clause.to_ground_inverse[OF D_grounding]
+                      clause.is_welltyped.subst_stability[OF \<rho>\<^sub>2_\<gamma>_is_welltyped].
+
+                  then obtain \<tau> where
+                    "welltyped \<V>\<^sub>2 (term.from_ground t\<^sub>G\<^sub>1) \<tau>"
+                    "welltyped \<V>\<^sub>2 (term.from_ground t\<^sub>G\<^sub>3) \<tau>"
+                    unfolding ground_superpositionI
+                    by auto
+
+                  then show ?thesis
+                    using that welltyped.explicit_replace_\<V>_iff[of _ \<V>\<^sub>2 \<V>\<^sub>1]
+                    by simp
+                qed
+
+                 ultimately show ?thesis
+                  by auto              
+              qed
+
+              moreover have "is_welltyped_on (\<Union> (term.vars ` \<rho>\<^sub>1 ` clause.vars E)) \<V>\<^sub>1 \<gamma>"
+                by (intro is_welltyped_on_subst_compose_renaming \<rho>\<^sub>1_\<gamma>_is_welltyped
+                    \<rho>\<^sub>1_is_welltyped \<rho>\<^sub>1)
+
+              ultimately show "is_welltyped_on (\<Union> (term.vars ` \<rho>\<^sub>1 ` clause.vars E)) \<V>\<^sub>1 \<gamma>'"
+                unfolding \<gamma>'_def
+                by simp
+            qed
+          qed
+
+          then show ?thesis
+            by simp
+        qed
+
+        show "finite {?E\<^sub>G'}"
+          by simp
+     
+        show "ground.G_entails ({?E\<^sub>G'} \<union> {D\<^sub>G}) {C\<^sub>G}"
+        proof(unfold ground.G_entails_def, intro allI impI)
+          fix I :: "'f gterm rel"
+          let ?I = "upair ` I"
+
+          assume 
+            refl_I: "refl I" and 
+            trans_I: "trans I" and 
+            sym_I: "sym I" and
+            compatible_with_gctxt_I: "compatible_with_gctxt I" and
+            premise: "?I \<TTurnstile>s {?E\<^sub>G'} \<union> {D\<^sub>G}"
+
+           then interpret clause_entailment I
+             by unfold_locales
+
+          have \<gamma>_x_is_ground: "term.is_ground (\<gamma> x)"
+            using t\<^sub>1_\<gamma> t\<^sub>1_\<rho>\<^sub>1
+            by auto
+
+          show "?I \<TTurnstile>s {C\<^sub>G}"
+          proof(cases "?I \<TTurnstile> D\<^sub>G'")
+            case True
+
+            then show ?thesis
+              unfolding ground_superpositionI
+              by auto
+          next
+            case False
+
+            then have t\<^sub>G\<^sub>1_t\<^sub>G\<^sub>3: "Upair t\<^sub>G\<^sub>1 t\<^sub>G\<^sub>3 \<in> ?I"
+              using premise sym
+              unfolding ground_superpositionI
+              by auto
+
+            have "?I \<TTurnstile>l c\<^sub>G'\<langle>t\<^sub>G\<^sub>1\<rangle>\<^sub>G \<approx> c\<^sub>G'\<langle>t\<^sub>G\<^sub>3\<rangle>\<^sub>G"
+              using upair_compatible_with_gctxtI[OF t\<^sub>G\<^sub>1_t\<^sub>G\<^sub>3]
+              by auto
+
+            then have "?I \<TTurnstile>l term.to_ground (t\<^sub>1 \<cdot>t \<rho>\<^sub>1 \<odot> \<gamma>) \<approx> term.to_ground (t\<^sub>1 \<cdot>t \<rho>\<^sub>1 \<odot> \<gamma>')"
+              unfolding t\<^sub>1_\<gamma> t\<^sub>1_\<gamma>'
+              by simp
+
+            then have "(term.to_ground (\<gamma> x), c\<^sub>G'\<langle>t\<^sub>G\<^sub>3\<rangle>\<^sub>G) \<in> I"
+              unfolding \<gamma>'_def
+              using t\<^sub>1_\<rho>\<^sub>1
+              by (auto simp: sym)
+
+            moreover have "?I \<TTurnstile> ?E\<^sub>G'"
+              using premise
+              by simp
+
+            ultimately have "?I \<TTurnstile> E\<^sub>G"
+              unfolding \<gamma>'_def E\<^sub>G
+              using
+                clause.symmetric_congruence[of _ \<gamma>, OF _ \<gamma>_x_is_ground]
+                E_grounding
+              by simp
+
+            then have "?I \<TTurnstile> add_mset (\<P>\<^sub>G (Upair c\<^sub>G\<langle>t\<^sub>G\<^sub>3\<rangle>\<^sub>G t\<^sub>G\<^sub>2)) E\<^sub>G'"
+              unfolding ground_superpositionI
+              using symmetric_literal_context_congruence[OF t\<^sub>G\<^sub>1_t\<^sub>G\<^sub>3]
+              by (cases "\<P>\<^sub>G = Pos") simp_all
+
+            then show ?thesis
+              unfolding ground_superpositionI
+              by blast
+          qed
+        qed
+
+        show "\<forall>E\<^sub>G' \<in> {?E\<^sub>G'}. E\<^sub>G' \<prec>\<^sub>c\<^sub>G E\<^sub>G"
+        proof-
+
+          have "\<gamma> x = t\<^sub>1 \<cdot>t \<rho>\<^sub>1 \<odot> \<gamma>"
+            using t\<^sub>1_\<rho>\<^sub>1
+            by simp
+
+          then have t\<^sub>G_smaller: "?t\<^sub>G \<prec>\<^sub>t \<gamma> x"
+            using ground_superpositionI(8)
+            unfolding t\<^sub>1_\<gamma> term.order.less\<^sub>G_def
+            by simp
+
+          have "?E\<^sub>G' \<prec>\<^sub>c\<^sub>G E\<^sub>G"
+          proof -
+
+            have "add_mset (l\<^sub>1 \<cdot>l \<rho>\<^sub>1 \<odot> \<gamma>') (E' \<cdot> \<rho>\<^sub>1 \<odot> \<gamma>') \<prec>\<^sub>c add_mset (l\<^sub>1 \<cdot>l \<rho>\<^sub>1 \<odot> \<gamma>) (E' \<cdot> \<rho>\<^sub>1 \<odot> \<gamma>)"
+            proof(rule less\<^sub>c_add_mset)
+
+              have "x \<in> literal.vars (l\<^sub>1 \<cdot>l \<rho>\<^sub>1)"
+                unfolding l\<^sub>1 c\<^sub>1_t\<^sub>1 literal.vars_def atom.vars_def 
+                using t\<^sub>1_\<rho>\<^sub>1
+                by auto
+
+              moreover have "literal.is_ground (l\<^sub>1 \<cdot>l \<rho>\<^sub>1 \<odot> \<gamma>)"
+                using E_grounding
+                unfolding E
+                by simp
+
+              ultimately show "l\<^sub>1 \<cdot>l \<rho>\<^sub>1 \<odot> \<gamma>' \<prec>\<^sub>l l\<^sub>1 \<cdot>l \<rho>\<^sub>1 \<odot> \<gamma>"
+                unfolding \<gamma>'_def
+                using literal.order.subst_update_stability t\<^sub>G_smaller
+                by simp
+            next
+
+              have "clause.is_ground (E' \<cdot> \<rho>\<^sub>1 \<odot> \<gamma>)"
+                using E'_\<gamma>
+                by simp
+
+              then show "E' \<cdot> \<rho>\<^sub>1 \<odot> \<gamma>' \<preceq>\<^sub>c E' \<cdot> \<rho>\<^sub>1 \<odot> \<gamma>"
+                unfolding \<gamma>'_def
+                using clause.order.subst_update_stability t\<^sub>G_smaller
+                by (cases "x \<in> clause.vars (E' \<cdot> \<rho>\<^sub>1)") simp_all
+            qed
+
+            then have "E \<cdot> \<rho>\<^sub>1 \<odot> \<gamma>' \<prec>\<^sub>c E \<cdot> \<rho>\<^sub>1 \<odot> \<gamma>"
+              unfolding E
+              by simp
+
+            moreover have "clause.is_ground (E \<cdot> \<rho>\<^sub>1 \<odot> \<gamma>')"
+              unfolding \<gamma>'_def
+              using E_grounding
+              by simp
+
+            ultimately show ?thesis
+              using E_grounding
+              unfolding clause.order.less\<^sub>G_def E\<^sub>G
+              by simp
+          qed
 
           then show ?thesis
             by blast
-        qed
+        qed   
       qed
+
+    qed
+
+    then show ?thesis
+      using non_redundant ground_superposition that l\<^sub>1 t\<^sub>1'_\<gamma> c\<^sub>1_t\<^sub>1_\<gamma> 
+      unfolding ground.Red_I_def ground.G_Inf_def
+      by auto
+  qed
+
+  obtain l\<^sub>2 where 
+    l\<^sub>2_\<gamma>: "l\<^sub>2 \<cdot>l \<rho>\<^sub>2 \<odot> \<gamma> = literal.from_ground l\<^sub>G\<^sub>2" and
+    l\<^sub>2_is_strictly_maximal: "is_strictly_maximal l\<^sub>2 D"
+  proof-
+    have "is_strictly_maximal (literal.from_ground l\<^sub>G\<^sub>2) (D \<cdot> \<rho>\<^sub>2 \<odot> \<gamma>)"
+      using ground_superpositionI(11) D_grounding
+      by simp
+
+    then show ?thesis
+      using obtain_strictly_maximal_literal[OF D_grounding] that
+      by metis
+  qed
+
+  then have l\<^sub>2_in_D: "l\<^sub>2 \<in># D" 
+    using strictly_maximal_in_clause 
+    by blast
+
+  from l\<^sub>2_\<gamma> have l\<^sub>2_\<gamma>: "l\<^sub>2 \<cdot>l \<rho>\<^sub>2 \<odot> \<gamma> = term.from_ground t\<^sub>G\<^sub>1 \<approx> term.from_ground t\<^sub>G\<^sub>3"
+    unfolding ground_superpositionI
+    by simp
+
+  then obtain t\<^sub>2 t\<^sub>2' where
+    l\<^sub>2: "l\<^sub>2 = t\<^sub>2 \<approx> t\<^sub>2'" and
+    t\<^sub>2_\<gamma>: "t\<^sub>2 \<cdot>t \<rho>\<^sub>2 \<odot> \<gamma> = term.from_ground t\<^sub>G\<^sub>1" and     
+    t\<^sub>2'_\<gamma>: "t\<^sub>2' \<cdot>t \<rho>\<^sub>2 \<odot> \<gamma> = term.from_ground t\<^sub>G\<^sub>3"
+    using obtain_from_pos_literal_subst
+    by metis
+
+  obtain D' where D: "D = add_mset l\<^sub>2 D'"
+    by (meson l\<^sub>2_in_D multi_member_split)
+
+  then have D'_\<gamma>: "D' \<cdot> \<rho>\<^sub>2 \<odot> \<gamma> = clause.from_ground D\<^sub>G'"
+    using D_\<gamma> l\<^sub>2_\<gamma>
+    unfolding ground_superpositionI
+    by auto
+
+  (* TODO: inv *) 
+  define \<V>\<^sub>3 where 
+    "\<And>x. \<V>\<^sub>3 x \<equiv>
+        if x \<in> clause.vars (E \<cdot> \<rho>\<^sub>1)
+        then \<V>\<^sub>1 (inv \<rho>\<^sub>1 (Var x))
+        else \<V>\<^sub>2 (inv \<rho>\<^sub>2 (Var x))"
+
+  have \<gamma>_is_welltyped: "is_welltyped_on (clause.vars (E \<cdot> \<rho>\<^sub>1) \<union> clause.vars (D \<cdot> \<rho>\<^sub>2)) \<V>\<^sub>3 \<gamma>"
+  proof(unfold Set.ball_Un, intro conjI)
+
+    show "is_welltyped_on (clause.vars (E \<cdot> \<rho>\<^sub>1)) \<V>\<^sub>3 \<gamma>"
+      unfolding \<V>\<^sub>3_def
+      using clause.is_welltyped.is_typed_on_renaming_grounding[OF \<rho>\<^sub>1 \<rho>\<^sub>1_\<gamma>_is_welltyped E_grounding]
+      by simp
+
+  next
+    have "\<forall>x\<in>clause.vars (D \<cdot> \<rho>\<^sub>2). \<V>\<^sub>3 x = \<V>\<^sub>2 (inv \<rho>\<^sub>2 (Var x))"
+      unfolding \<V>\<^sub>3_def
+      using rename_apart
+      by auto
+
+    then show "is_welltyped_on (clause.vars (D \<cdot> \<rho>\<^sub>2)) \<V>\<^sub>3 \<gamma>"
+      unfolding \<V>\<^sub>3_def
+      using clause.is_welltyped.is_typed_on_renaming_grounding[OF \<rho>\<^sub>2 \<rho>\<^sub>2_\<gamma>_is_welltyped D_grounding]
+      by simp
+  qed
+
+  obtain \<mu> \<sigma> where \<mu>: 
+    "term_subst.is_imgu \<mu> {{t\<^sub>1 \<cdot>t \<rho>\<^sub>1, t\<^sub>2 \<cdot>t \<rho>\<^sub>2}}" 
+    "\<gamma> = \<mu> \<odot> \<sigma>" 
+    "welltyped_imgu \<V>\<^sub>3 (t\<^sub>1 \<cdot>t \<rho>\<^sub>1) (t\<^sub>2 \<cdot>t \<rho>\<^sub>2) \<mu>"
+  proof-
+
+    have unified: "t\<^sub>1 \<cdot>t \<rho>\<^sub>1 \<cdot>t \<gamma> = t\<^sub>2 \<cdot>t \<rho>\<^sub>2 \<cdot>t \<gamma>"
+      using t\<^sub>1_\<gamma> t\<^sub>2_\<gamma> 
+      by simp
+
+    obtain \<tau> where welltyped: "welltyped \<V>\<^sub>3 (t\<^sub>1 \<cdot>t \<rho>\<^sub>1) \<tau>" "welltyped \<V>\<^sub>3 (t\<^sub>2 \<cdot>t \<rho>\<^sub>2) \<tau>"
+    proof-
+      have "clause.is_welltyped \<V>\<^sub>2 (D \<cdot> \<rho>\<^sub>2 \<odot> \<gamma>)"
+        using \<rho>\<^sub>2_\<gamma>_is_welltyped D_is_welltyped
+        by (metis clause.is_welltyped.subst_stability)
+
+      then obtain \<tau> where 
+        "welltyped \<V>\<^sub>2 (term.from_ground t\<^sub>G\<^sub>1) \<tau>" 
+        unfolding D_\<gamma> ground_superpositionI
+        by auto
+
+      then have 
+        "welltyped \<V>\<^sub>3 (term.from_ground t\<^sub>G\<^sub>1) \<tau>" 
+        using welltyped.is_ground_typed
+        by (meson term.ground_is_ground welltyped.explicit_is_ground_typed)
+
+      then have "welltyped \<V>\<^sub>3 (t\<^sub>1 \<cdot>t \<rho>\<^sub>1 \<odot> \<gamma>) \<tau>" "welltyped \<V>\<^sub>3 (t\<^sub>2 \<cdot>t \<rho>\<^sub>2 \<odot> \<gamma>) \<tau>"
+        using t\<^sub>1_\<gamma> t\<^sub>2_\<gamma>
+        by presburger+
+
+      moreover have
+        "term.vars (t\<^sub>1 \<cdot>t \<rho>\<^sub>1) \<subseteq> clause.vars (E \<cdot> \<rho>\<^sub>1)"
+        "term.vars (t\<^sub>2 \<cdot>t \<rho>\<^sub>2) \<subseteq> clause.vars (D \<cdot> \<rho>\<^sub>2)"
+        unfolding E l\<^sub>1 clause.add_subst D l\<^sub>2
+        by auto
+
+      ultimately have "welltyped \<V>\<^sub>3 (t\<^sub>1 \<cdot>t \<rho>\<^sub>1) \<tau>" "welltyped \<V>\<^sub>3 (t\<^sub>2 \<cdot>t \<rho>\<^sub>2) \<tau>"
+        using \<gamma>_is_welltyped
+        by (simp_all add: subsetD)
 
       then show ?thesis
         using that
         by blast
     qed
 
-    then have context\<^sub>G: "context.from_ground context\<^sub>G = context\<^sub>x \<circ>\<^sub>c context\<^sub>x' \<cdot>t\<^sub>c \<rho>\<^sub>1 \<cdot>t\<^sub>c \<gamma>"
-      using context.ground_context_subst[OF context.ground_is_ground] ctxt_compose_subst_compose_distrib
-      by metis
-
-    obtain \<tau>\<^sub>x where \<tau>\<^sub>x: "welltyped \<V>\<^sub>1 term\<^sub>x \<tau>\<^sub>x"
-      using term\<^sub>1_with_context typing(1)
-      unfolding premise\<^sub>1 literal\<^sub>1
-      by (metis welltyped.simps is_Var_term\<^sub>x term.collapse(1))
- 
-    have \<iota>\<^sub>G_parts: 
-      "set (side_prems_of \<iota>\<^sub>G) = {premise\<^sub>G\<^sub>2}" 
-      "main_prem_of \<iota>\<^sub>G = premise\<^sub>G\<^sub>1"
-      "concl_of \<iota>\<^sub>G = conclusion\<^sub>G"
-      unfolding \<iota>\<^sub>G
-      by simp_all
-
-    from is_Var_term\<^sub>x 
-    obtain var\<^sub>x where var\<^sub>x: "Var var\<^sub>x = term\<^sub>x \<cdot>t \<rho>\<^sub>1"
-      using renaming(1)
-      unfolding is_Var_def term_subst.is_renaming_def subst_compose_def
-      by (metis eval_subst_def eval_term.simps(1) term.is_renaming_def renaming(1) 
-          subst_apply_eq_Var)
-
-    have \<tau>\<^sub>x_var\<^sub>x: "welltyped \<V>\<^sub>1 (Var var\<^sub>x) \<tau>\<^sub>x"
-      using \<tau>\<^sub>x typing(5)
-      unfolding var\<^sub>x premise\<^sub>1 literal\<^sub>1 term\<^sub>1_with_context
-      by simp
-
     show ?thesis
-    proof(unfold ground.redundant_infer_def \<iota>\<^sub>G_parts, intro exI conjI)
-
-      let ?update = "(context\<^sub>x' \<cdot>t\<^sub>c \<rho>\<^sub>1 \<cdot>t\<^sub>c \<gamma>)\<langle>term.from_ground term\<^sub>G\<^sub>3\<rangle>"
-
-      define \<gamma>' where
-        \<gamma>': "\<gamma>' \<equiv> \<gamma>(var\<^sub>x := ?update)"
-
-      have update_grounding: "term.is_ground ?update"
-      proof-
-        have "context.is_ground ((context\<^sub>x \<cdot>t\<^sub>c \<rho>\<^sub>1 \<cdot>t\<^sub>c \<gamma>) \<circ>\<^sub>c (context\<^sub>x' \<cdot>t\<^sub>c \<rho>\<^sub>1 \<cdot>t\<^sub>c \<gamma>))"
-          using context.ground_is_ground[of context\<^sub>G] context\<^sub>G
-          by (metis subst_compose_ctxt_compose_distrib)
-
-        then show ?thesis
-          using context.context_is_ground_context_compose1(2)
-          by auto
-      qed
-      let ?context\<^sub>x'_\<gamma> = "context.to_ground (context\<^sub>x' \<cdot>t\<^sub>c \<rho>\<^sub>1 \<cdot>t\<^sub>c \<gamma>)"
-
-      (* TODO: *)
-      have term\<^sub>x_\<gamma>: "term.to_ground (term\<^sub>x \<cdot>t \<rho>\<^sub>1 \<cdot>t \<gamma>) = ?context\<^sub>x'_\<gamma>\<langle>term\<^sub>G\<^sub>1\<rangle>\<^sub>G"
-      proof-
-        have "(context\<^sub>x \<cdot>t\<^sub>c \<rho>\<^sub>1 \<cdot>t\<^sub>c \<gamma>)\<langle>term\<^sub>x \<cdot>t \<rho>\<^sub>1 \<cdot>t \<gamma>\<rangle> = 
-          (context\<^sub>x \<cdot>t\<^sub>c \<rho>\<^sub>1 \<cdot>t\<^sub>c \<gamma>) \<langle>(context\<^sub>x' \<cdot>t\<^sub>c \<rho>\<^sub>1 \<cdot>t\<^sub>c \<gamma>)\<langle>term.from_ground term\<^sub>G\<^sub>1\<rangle>\<rangle>"
-          using term\<^sub>1_with_context_\<gamma> 
-          unfolding term\<^sub>1_with_context context\<^sub>G
-          by (metis ctxt_ctxt_compose eval_ctxt subst_compose_ctxt_compose_distrib)
-        
-        then show ?thesis
-          using update_grounding 
-          by (metis ctxt_eq context.term_to_ground_context_to_ground term.from_ground_inverse)
-      qed
-
-      have term\<^sub>x_\<gamma>': "term.to_ground (term\<^sub>x \<cdot>t \<rho>\<^sub>1 \<cdot>t \<gamma>') = ?context\<^sub>x'_\<gamma>\<langle>term\<^sub>G\<^sub>3\<rangle>\<^sub>G"
-        using update_grounding
-        unfolding var\<^sub>x[symmetric] \<gamma>'
-        by auto
-
-      have aux: "term\<^sub>x \<cdot>t \<rho>\<^sub>1 \<cdot>t \<gamma> = (context\<^sub>x' \<cdot>t\<^sub>c \<rho>\<^sub>1 \<cdot>t\<^sub>c \<gamma>)\<langle>term.from_ground term\<^sub>G\<^sub>1\<rangle>"
-        using term\<^sub>x_\<gamma>
-        by (metis (mono_tags, lifting) context.ground_is_ground
-            context.term_from_ground_context_to_ground
-            context.term_with_context_is_ground subst_apply_term_ctxt_apply_distrib
-            term.to_ground_inverse term\<^sub>1_with_context term\<^sub>1_with_context_\<gamma> update_grounding
-            vars_term_of_gterm)
-
-      have "clause.is_welltyped \<V>\<^sub>2 (clause.from_ground premise\<^sub>G\<^sub>2)"
-        by (metis clause.comp_subst.monoid_action_compatibility clause.is_welltyped.subst_stability 
-            clause.to_ground_inverse premise\<^sub>2_grounding premise\<^sub>G\<^sub>2 typing(2,4))
-
-      then have 
-        "\<exists>\<tau>. welltyped \<V>\<^sub>2 (term.from_ground term\<^sub>G\<^sub>1) \<tau> \<and> welltyped \<V>\<^sub>2 (term.from_ground term\<^sub>G\<^sub>3) \<tau>"
-        unfolding ground_superpositionI 
-        by simp
-
-      then have aux': "\<exists>\<tau>. welltyped \<V>\<^sub>1 (term.from_ground term\<^sub>G\<^sub>1) \<tau> \<and> 
-          welltyped \<V>\<^sub>1 (term.from_ground term\<^sub>G\<^sub>3) \<tau>"
-        by (meson term.ground_is_ground welltyped.explicit_is_ground_typed)
-
-      have "welltyped \<V>\<^sub>1 (term\<^sub>x \<cdot>t \<rho>\<^sub>1 \<cdot>t \<gamma>) \<tau>\<^sub>x"
-      proof-
-
-        have "
-          \<lbrakk>\<forall>x\<in>context.vars context\<^sub>x \<union> term.vars term\<^sub>x \<union> term.vars term\<^sub>1' \<union> clause.vars premise\<^sub>1'.
-            welltyped \<V>\<^sub>1 ((\<rho>\<^sub>1 \<odot> \<gamma>) x) (\<V>\<^sub>1 x);
-            welltyped \<V>\<^sub>1 term\<^sub>x \<tau>\<^sub>x\<rbrakk>
-            \<Longrightarrow> welltyped \<V>\<^sub>1 (term\<^sub>x \<cdot>t \<rho>\<^sub>1 \<cdot>t \<gamma>) \<tau>\<^sub>x"
-          by (metis Un_iff term_subst.subst_comp_subst welltyped.explicit_subst_stability)
-        
-        then show ?thesis
-          using typing(3) \<tau>\<^sub>x
-          unfolding var\<^sub>x premise\<^sub>1 literal\<^sub>1 term\<^sub>1_with_context
-          by simp
-      qed
-
-      then have \<tau>\<^sub>x_update: "welltyped \<V>\<^sub>1 ?update \<tau>\<^sub>x"
-        unfolding aux
-        using aux'
-        by blast
-
-      let ?premise\<^sub>1_\<gamma>' = "clause.to_ground (premise\<^sub>1 \<cdot> \<rho>\<^sub>1 \<cdot> \<gamma>')"
-      have premise\<^sub>1_\<gamma>'_grounding: "clause.is_ground (premise\<^sub>1 \<cdot> \<rho>\<^sub>1 \<cdot> \<gamma>')"
-        using clause.ground_subst_update[OF update_grounding premise\<^sub>1_grounding] 
-        unfolding \<gamma>'
-        by blast
-
-      (*have \<gamma>'_ground: "term_subst.is_ground_subst (\<rho>\<^sub>1 \<odot> \<gamma>')"
-        sledgehammer
-        sorry*)
-        (*by (metis \<gamma>' term.ground_subst_update term_subst.comp_subst.left.monoid_action_compatibility 
-            term_subst.is_ground_subst_def typing(2) update_grounding)*)
-
-      have \<gamma>'_wt: "is_welltyped_on (clause.vars premise\<^sub>1) \<V>\<^sub>1 (\<rho>\<^sub>1 \<odot> \<gamma>')"
-        using welltyped.subst_update[OF \<tau>\<^sub>x_var\<^sub>x \<tau>\<^sub>x_update typing(3)]
-        unfolding \<gamma>' subst_compose
-        using welltyped.simps \<tau>\<^sub>x \<tau>\<^sub>x_update eval_term.simps(1) 
-          eval_with_fresh_var fun_upd_same is_Var_term\<^sub>x renaming(1) subst_compose_def 
-          term.collapse(1) term.distinct(1) term.set_cases(2) term_subst_is_renaming_iff 
-          the_inv_f_f typing(3) var\<^sub>x
-        by (smt (verit, del_insts))
-      
-      show "{?premise\<^sub>1_\<gamma>'} \<subseteq> premise_groundings"
-        using premise\<^sub>1_\<gamma>'_grounding typing \<gamma>'_wt
-        unfolding clause.subst_comp_subst[symmetric] premise\<^sub>1 premise_groundings 
-          clause_groundings_def
-        by (smt (verit, ccfv_threshold) Un_iff empty_iff fst_conv insert_iff mem_Collect_eq snd_conv subset_iff)
-
-      show "finite {?premise\<^sub>1_\<gamma>'}"
-        by simp
-
-      show "ground.G_entails ({?premise\<^sub>1_\<gamma>'} \<union> {premise\<^sub>G\<^sub>2}) {conclusion\<^sub>G}"
-      proof(unfold ground.G_entails_def, intro allI impI)
-        fix I :: "'f gterm rel"
-        let ?I = "upair ` I"
-
-        assume 
-          refl: "refl I" and 
-          trans: "trans I" and 
-          sym: "sym I" and
-          compatible_with_gctxt: "compatible_with_gctxt I" and
-          premise: "?I \<TTurnstile>s {?premise\<^sub>1_\<gamma>'} \<union> {premise\<^sub>G\<^sub>2}"
-
-        interpret clause_entailment I
-          by unfold_locales (rule trans sym compatible_with_gctxt)+
-
-        have var\<^sub>x_\<gamma>_ground: "term.is_ground (\<gamma> var\<^sub>x)"
-          using term\<^sub>1_with_context_\<gamma>
-          unfolding term\<^sub>1_with_context var\<^sub>x
-          by (metis aux eval_term.simps(1) nonground_context.term_with_context_is_ground
-              term.ground_is_ground update_grounding var\<^sub>x)
-
-        show "?I \<TTurnstile>s { conclusion\<^sub>G }"
-        proof(cases "?I \<TTurnstile> premise\<^sub>G\<^sub>2'")
-          case True
-          then show ?thesis 
-            unfolding ground_superpositionI(12)
-            by auto
-        next
-          case False
-          then have literal\<^sub>G\<^sub>2: "?I \<TTurnstile>l literal\<^sub>G\<^sub>2"
-            using premise 
-            unfolding ground_superpositionI(2)
-            by blast
-
-          then have "?I \<TTurnstile>l ?context\<^sub>x'_\<gamma>\<langle>term\<^sub>G\<^sub>1\<rangle>\<^sub>G \<approx> ?context\<^sub>x'_\<gamma>\<langle>term\<^sub>G\<^sub>3\<rangle>\<^sub>G"
-            unfolding ground_superpositionI(6)
-            using compatible_with_gctxt compatible_with_gctxt_def sym 
-            by auto
-
-          then have "?I \<TTurnstile>l term.to_ground (term\<^sub>x \<cdot>t \<rho>\<^sub>1 \<cdot>t \<gamma>) \<approx> term.to_ground (term\<^sub>x \<cdot>t \<rho>\<^sub>1 \<cdot>t \<gamma>')"
-            using term\<^sub>x_\<gamma> term\<^sub>x_\<gamma>'
-            by argo
-
-          then have "(term.to_ground (\<gamma> var\<^sub>x), 
-                      term.to_ground (context\<^sub>x' \<cdot>t\<^sub>c \<rho>\<^sub>1 \<cdot>t\<^sub>c \<gamma>)\<langle>term.from_ground term\<^sub>G\<^sub>3\<rangle>) \<in> I"
-            unfolding \<gamma>'
-            using var\<^sub>x
-            by(auto simp: sym)
-        
-          moreover then have "?I \<TTurnstile> ?premise\<^sub>1_\<gamma>'"
-            using premise by fastforce
-
-          ultimately have "?I \<TTurnstile> premise\<^sub>G\<^sub>1"
-            using
-              clause.symmetric_congruence[of _ \<gamma>, 
-                                          OF update_grounding var\<^sub>x_\<gamma>_ground _ premise\<^sub>1_grounding]
-            unfolding \<gamma>' premise\<^sub>G\<^sub>1
-            by blast
-
-          then have "?I \<TTurnstile> add_mset (\<P>\<^sub>G (Upair context\<^sub>G\<langle>term\<^sub>G\<^sub>1\<rangle>\<^sub>G term\<^sub>G\<^sub>2)) premise\<^sub>G\<^sub>1'"
-            using ground_superpositionI(1) ground_superpositionI(5) by auto
-
-          then have "?I \<TTurnstile> add_mset (\<P>\<^sub>G (Upair context\<^sub>G\<langle>term\<^sub>G\<^sub>3\<rangle>\<^sub>G term\<^sub>G\<^sub>2)) premise\<^sub>G\<^sub>1'"
-            using literal\<^sub>G\<^sub>2 symmetric_context_congruence ground_superpositionI(4)
-            unfolding ground_superpositionI(6)
-            apply(cases "\<P>\<^sub>G = Pos")
-            (* TODO: Probably Upair_Extra was auto simp: sym *)
-             apply(auto )
-                   apply blast
-                  apply(auto simp: sym)
-            by (meson local.sym symD)+
-
-          then show ?thesis 
-            unfolding ground_superpositionI(12)
-            by blast
-        qed
-      qed
-
-      show "\<forall>clause\<^sub>G \<in> {?premise\<^sub>1_\<gamma>'}. clause\<^sub>G \<prec>\<^sub>c\<^sub>G premise\<^sub>G\<^sub>1"
-      proof-
-        have var\<^sub>x_\<gamma>: "\<gamma> var\<^sub>x = term\<^sub>x \<cdot>t \<rho>\<^sub>1 \<cdot>t \<gamma>"
-          using var\<^sub>x
-          by simp
-
-        have context\<^sub>x_grounding: "context.is_ground (context\<^sub>x \<cdot>t\<^sub>c \<rho>\<^sub>1 \<cdot>t\<^sub>c \<gamma>)"
-          using context\<^sub>G
-          unfolding subst_compose_ctxt_compose_distrib
-          by (metis context.ground_is_ground context.context_is_ground_context_compose1(1))
-
-        have term\<^sub>x_grounding: "term.is_ground (term\<^sub>x \<cdot>t \<rho>\<^sub>1 \<cdot>t \<gamma>)"
-          using term\<^sub>1_with_context_\<gamma>
-          unfolding term\<^sub>1_with_context
-          by (metis aux nonground_context.term_with_context_is_ground term.ground_is_ground
-              update_grounding)
-
-        have 
-          "(context\<^sub>x \<circ>\<^sub>c context\<^sub>x' \<cdot>t\<^sub>c \<rho>\<^sub>1 \<cdot>t\<^sub>c \<gamma>)\<langle>term.from_ground term\<^sub>G\<^sub>3\<rangle> \<prec>\<^sub>t context\<^sub>x\<langle>term\<^sub>x\<rangle> \<cdot>t \<rho>\<^sub>1 \<cdot>t \<gamma>"
-          using ground_superpositionI(8)
-          unfolding 
-            term.order.less\<^sub>G_def 
-            context\<^sub>G[symmetric] 
-            term\<^sub>1_with_context[symmetric] 
-            term\<^sub>1_with_context_\<gamma>
-          by (simp add: term.order.ground_context_compatibility)
-
-        then have update_smaller: "?update \<prec>\<^sub>t \<gamma> var\<^sub>x"
-          unfolding 
-            var\<^sub>x_\<gamma>
-            subst_apply_term_ctxt_apply_distrib 
-            subst_compose_ctxt_compose_distrib
-            Subterm_and_Context.ctxt_ctxt_compose
-          using term.order.context_compatibility[OF 
-              update_grounding term\<^sub>x_grounding context\<^sub>x_grounding]
-          by simp   
-
-        have var\<^sub>x_in_literal\<^sub>1: "var\<^sub>x \<in> literal.vars (literal\<^sub>1 \<cdot>l \<rho>\<^sub>1)"
-          unfolding literal\<^sub>1 term\<^sub>1_with_context literal.vars_def atom.vars_def 
-          using var\<^sub>x
-          by auto
-
-        have literal\<^sub>1_smaller: "literal\<^sub>1 \<cdot>l \<rho>\<^sub>1 \<cdot>l \<gamma>' \<prec>\<^sub>l literal\<^sub>1 \<cdot>l \<rho>\<^sub>1 \<cdot>l \<gamma>"
-          unfolding \<gamma>'
-          using literal.order.subst_update_stability[OF 
-              update_grounding 
-              update_smaller 
-              literal\<^sub>1_grounding[unfolded literal.subst_comp_subst] 
-              var\<^sub>x_in_literal\<^sub>1
-              ].
-
-        have premise\<^sub>1'_grounding: "clause.is_ground (premise\<^sub>1' \<cdot> \<rho>\<^sub>1 \<cdot> \<gamma>)"
-          using premise\<^sub>1'_\<gamma>
-          by simp
-
-        have premise\<^sub>1'_smaller: "premise\<^sub>1' \<cdot> \<rho>\<^sub>1 \<cdot> \<gamma>' \<preceq>\<^sub>c premise\<^sub>1' \<cdot> \<rho>\<^sub>1 \<cdot> \<gamma>"
-          unfolding \<gamma>'
-          using clause.order.subst_update_stability[of _ \<gamma>, OF update_grounding update_smaller premise\<^sub>1'_grounding]
-          by(cases "var\<^sub>x \<in> clause.vars (premise\<^sub>1' \<cdot> \<rho>\<^sub>1)") simp_all
-
-        have "?premise\<^sub>1_\<gamma>' \<prec>\<^sub>c\<^sub>G premise\<^sub>G\<^sub>1"
-          using less\<^sub>c_add_mset[OF literal\<^sub>1_smaller premise\<^sub>1'_smaller]
-          unfolding 
-            clause.order.less\<^sub>G_def 
-            premise\<^sub>G\<^sub>1
-            clause.add_subst[symmetric]
-            clause.to_ground_inverse[OF premise\<^sub>1_\<gamma>'_grounding]
-            clause.to_ground_inverse[OF premise\<^sub>1_grounding]
-          unfolding premise\<^sub>1.
-
-        then show ?thesis
-          by blast
-      qed   
-    qed
+      using obtain_welltyped_imgu[OF unified welltyped] that
+      by metis
   qed
 
-  obtain context\<^sub>1 term\<^sub>1 where 
-    term\<^sub>1_with_context: "term\<^sub>1_with_context = context\<^sub>1\<langle>term\<^sub>1\<rangle>" and
-    term\<^sub>1_\<gamma>: "term\<^sub>1 \<cdot>t \<rho>\<^sub>1 \<cdot>t \<gamma> = term.from_ground term\<^sub>G\<^sub>1" and
-    context\<^sub>1_\<gamma>: "context\<^sub>1 \<cdot>t\<^sub>c \<rho>\<^sub>1 \<cdot>t\<^sub>c \<gamma> = context.from_ground context\<^sub>G" and
-    term\<^sub>1_not_Var: "\<not> is_Var term\<^sub>1"
-    using non_redundant ground_superposition inference_into_var_is_redundant 
-    unfolding
-      ground.Red_I_def 
-      ground.G_Inf_def 
-      premise_groundings 
-      \<iota>\<^sub>G 
-      conclusion\<^sub>G 
-      ground_superpositionI(1, 2) 
-      premise_groundings 
-    by blast
-
-  obtain term\<^sub>2'_with_context where 
-    term\<^sub>2'_with_context_\<gamma>: 
-      "term\<^sub>2'_with_context \<cdot>t \<gamma> = (context.from_ground context\<^sub>G)\<langle>term.from_ground term\<^sub>G\<^sub>3\<rangle>" and
-    term\<^sub>2'_with_context: "term\<^sub>2'_with_context = (context\<^sub>1 \<cdot>t\<^sub>c \<rho>\<^sub>1)\<langle>term\<^sub>2' \<cdot>t \<rho>\<^sub>2\<rangle>" 
-    unfolding term\<^sub>2'_\<gamma>[symmetric] context\<^sub>1_\<gamma>[symmetric]
+  have (* TODO: Separate *)
+    c\<^sub>1_t\<^sub>2'_\<gamma>: "(c\<^sub>1 \<cdot>t\<^sub>c \<rho>\<^sub>1)\<langle>t\<^sub>2' \<cdot>t \<rho>\<^sub>2\<rangle> \<cdot>t \<gamma> = (context.from_ground c\<^sub>G)\<langle>term.from_ground t\<^sub>G\<^sub>3\<rangle>"
+    unfolding t\<^sub>2'_\<gamma>[symmetric] c\<^sub>1_\<gamma>[symmetric]
     by force
 
-  define \<V>\<^sub>3 where 
-    "\<And>x. \<V>\<^sub>3 x \<equiv>
-        if x \<in> clause.vars (premise\<^sub>1 \<cdot> \<rho>\<^sub>1)
-        then \<V>\<^sub>1 (inv \<rho>\<^sub>1 (Var x))
-        else \<V>\<^sub>2 (inv \<rho>\<^sub>2 (Var x))"
+  
 
-  have wt_\<gamma>: 
-    "is_welltyped_on (clause.vars (premise\<^sub>1 \<cdot> \<rho>\<^sub>1) \<union> clause.vars (premise\<^sub>2 \<cdot> \<rho>\<^sub>2)) \<V>\<^sub>3 \<gamma>"
-  proof(intro ballI)
-    fix x
-    assume x_in_vars: "x \<in> clause.vars (premise\<^sub>1 \<cdot> \<rho>\<^sub>1) \<union> clause.vars (premise\<^sub>2 \<cdot> \<rho>\<^sub>2)"
+  
 
-    then have "term.is_ground (\<gamma> x)"
-      using premise\<^sub>1_grounding premise\<^sub>2_grounding
-      by (auto simp: clause.variable_grounding)
+ 
 
-    then obtain f ts where \<gamma>_x: "\<gamma> x = Fun f ts"
-      using term.obtain_ground_fun 
-      by blast
-
-    have "welltyped \<V>\<^sub>3 (\<gamma> x) (\<V>\<^sub>3 x)"
-    proof(cases "x \<in> clause.vars (premise\<^sub>1 \<cdot> \<rho>\<^sub>1)")
-      case True
-      then have "Var x \<in> \<rho>\<^sub>1 ` clause.vars premise\<^sub>1"
-        by (metis image_eqI renaming(1) clause.renaming_variables)
-
-      then have y_in_vars: "inv \<rho>\<^sub>1 (Var x) \<in> clause.vars premise\<^sub>1"
-        by (metis (no_types, lifting) image_iff renaming(1) term_subst_is_renaming_iff inv_f_f)
-
-      define y where "y \<equiv> inv \<rho>\<^sub>1 (Var x)"
-
-      have "term.is_ground (Var y \<cdot>t \<rho>\<^sub>1 \<cdot>t \<gamma>)"
-        by (metis (no_types, lifting) clause.subst_comp_subst clause.variable_grounding
-            eval_subst eval_term.simps(1) premise\<^sub>1_grounding y_def y_in_vars)
-
-      moreover have "welltyped \<V>\<^sub>1 (Var y \<cdot>t \<rho>\<^sub>1 \<cdot>t \<gamma>) (\<V>\<^sub>1 y)"
-        using typing(3) y_in_vars
-        unfolding y_def
-        by (simp add: subst_compose)
-
-      ultimately have "welltyped \<V>\<^sub>3 (Var y \<cdot>t \<rho>\<^sub>1 \<cdot>t \<gamma>) (\<V>\<^sub>1 y)"
-        by (meson welltyped.explicit_is_ground_typed)
-
-      moreover have "\<rho>\<^sub>1 (inv \<rho>\<^sub>1 (Var x)) = Var x"
-        by (metis \<open>Var x \<in> \<rho>\<^sub>1 ` clause.vars premise\<^sub>1\<close> image_iff renaming(1) term_subst_is_renaming_iff inv_f_f)
-
-      ultimately show ?thesis
-        using True
-        unfolding \<V>\<^sub>3_def y_def
-        by simp
-    next
-      case False
-      then have "Var x \<in> \<rho>\<^sub>2 ` clause.vars premise\<^sub>2"
-        using x_in_vars
-        by (metis Un_iff image_eqI renaming(2) clause.renaming_variables)
-
-      then have y_in_vars: "inv \<rho>\<^sub>2 (Var x) \<in> clause.vars premise\<^sub>2"
-        by (metis (no_types, lifting) image_iff renaming(2) term_subst_is_renaming_iff inv_f_f)
-
-      define y where "y \<equiv> inv \<rho>\<^sub>2 (Var x)"
-
-      have "term.is_ground (Var y \<cdot>t \<rho>\<^sub>2 \<cdot>t \<gamma>)"
-        by (metis (no_types, lifting) clause.comp_subst.left.monoid_action_compatibility
-            clause.variable_grounding eval_subst eval_term.simps(1) premise\<^sub>2_grounding y_def
-            y_in_vars)
-
-      moreover have "welltyped \<V>\<^sub>2 (Var y \<cdot>t \<rho>\<^sub>2 \<cdot>t \<gamma>) (\<V>\<^sub>2 y)"
-        using typing(4) y_in_vars
-        unfolding y_def
-        by (simp add: subst_compose)
-
-      ultimately have "welltyped \<V>\<^sub>3 (Var y \<cdot>t \<rho>\<^sub>2 \<cdot>t \<gamma>) (\<V>\<^sub>2 y)"
-        by (meson welltyped.explicit_is_ground_typed)     
-
-      moreover have "\<rho>\<^sub>2 (inv \<rho>\<^sub>2 (Var x)) = Var x"
-        by (metis \<open>Var x \<in> \<rho>\<^sub>2 ` clause.vars premise\<^sub>2\<close> image_iff renaming(2) 
-            term_subst_is_renaming_iff inv_f_f)
-
-      ultimately show ?thesis
-        using False
-        unfolding \<V>\<^sub>3_def y_def
-        by simp
-    qed
-
-    then show "welltyped \<V>\<^sub>3 (\<gamma> x) (\<V>\<^sub>3 x)"
-      unfolding \<gamma>_x.
-  qed
-
-  have "term\<^sub>1 \<cdot>t \<rho>\<^sub>1 \<cdot>t \<gamma> = term\<^sub>2 \<cdot>t \<rho>\<^sub>2 \<cdot>t \<gamma>"
-    unfolding term\<^sub>1_\<gamma> term\<^sub>2_\<gamma> ..
-
-  moreover have  "\<exists>\<tau>. welltyped \<V>\<^sub>3 (term\<^sub>1 \<cdot>t \<rho>\<^sub>1) \<tau> \<and> welltyped \<V>\<^sub>3 (term\<^sub>2 \<cdot>t \<rho>\<^sub>2) \<tau>"
-  proof-
-    have "clause.is_welltyped  \<V>\<^sub>2 (premise\<^sub>2 \<cdot> \<rho>\<^sub>2 \<cdot> \<gamma>)"
-      using typing
-      by (metis clause.comp_subst.monoid_action_compatibility clause.is_welltyped.subst_stability)
-
-    then obtain \<tau> where 
-      "welltyped \<V>\<^sub>2 (term.from_ground term\<^sub>G\<^sub>1) \<tau>" 
-      unfolding premise\<^sub>2_\<gamma> ground_superpositionI
-      by auto
-
-    then have 
-      "welltyped \<V>\<^sub>3 (term.from_ground term\<^sub>G\<^sub>1) \<tau>" 
-      using welltyped.is_ground_typed
-      by (meson term.ground_is_ground welltyped.explicit_is_ground_typed)
-
-    then have "welltyped \<V>\<^sub>3 (term.from_ground term\<^sub>G\<^sub>1) \<tau>"
-      by auto
-
-    then have "welltyped \<V>\<^sub>3 (term\<^sub>1 \<cdot>t \<rho>\<^sub>1 \<cdot>t \<gamma>) \<tau>" "welltyped \<V>\<^sub>3 (term\<^sub>2 \<cdot>t \<rho>\<^sub>2 \<cdot>t \<gamma>) \<tau>"
-      using term\<^sub>1_\<gamma> term\<^sub>2_\<gamma>
-      by presburger+
-
-    moreover have 
-      "term.vars (term\<^sub>1 \<cdot>t \<rho>\<^sub>1) \<subseteq> clause.vars (premise\<^sub>1 \<cdot> \<rho>\<^sub>1)"
-      "term.vars (term\<^sub>2 \<cdot>t \<rho>\<^sub>2) \<subseteq> clause.vars (premise\<^sub>2 \<cdot> \<rho>\<^sub>2)"
-      unfolding premise\<^sub>1 literal\<^sub>1 clause.add_subst term\<^sub>1_with_context premise\<^sub>2 literal\<^sub>2
-      by auto
-
-    ultimately have "welltyped \<V>\<^sub>3 (term\<^sub>1 \<cdot>t \<rho>\<^sub>1) \<tau>" "welltyped \<V>\<^sub>3 (term\<^sub>2 \<cdot>t \<rho>\<^sub>2) \<tau>"
-      using wt_\<gamma>
-      by (simp_all add: subsetD)+ 
-
-    then show ?thesis
-      by blast
-  qed
-
-  ultimately obtain \<mu> \<sigma> where \<mu>: 
-    "term_subst.is_imgu \<mu> {{term\<^sub>1 \<cdot>t \<rho>\<^sub>1, term\<^sub>2 \<cdot>t \<rho>\<^sub>2}}" 
-    "\<gamma> = \<mu> \<odot> \<sigma>" 
-    "welltyped_imgu \<V>\<^sub>3 (term\<^sub>1 \<cdot>t \<rho>\<^sub>1) (term\<^sub>2 \<cdot>t \<rho>\<^sub>2) \<mu>"
-    using welltyped_imgu_exists
-    by (smt (verit, del_insts))
-
-  define conclusion' where 
-    conclusion': "conclusion' \<equiv>
-      add_mset (?\<P> (Upair term\<^sub>2'_with_context (term\<^sub>1' \<cdot>t \<rho>\<^sub>1))) (premise\<^sub>1' \<cdot> \<rho>\<^sub>1 + premise\<^sub>2' \<cdot> \<rho>\<^sub>2) \<cdot> \<mu>"
+  define C' where 
+    C': "C' \<equiv>
+      add_mset (?\<P> (Upair (c\<^sub>1 \<cdot>t\<^sub>c \<rho>\<^sub>1)\<langle>t\<^sub>2' \<cdot>t \<rho>\<^sub>2\<rangle> (t\<^sub>1' \<cdot>t \<rho>\<^sub>1))) (E' \<cdot> \<rho>\<^sub>1 + D' \<cdot> \<rho>\<^sub>2) \<cdot> \<mu>"
 
   show ?thesis
   proof(rule that)
-    show "superposition (premise\<^sub>2, \<V>\<^sub>2) (premise\<^sub>1, \<V>\<^sub>1) (conclusion', \<V>\<^sub>3)"
+    show "superposition (D, \<V>\<^sub>2) (E, \<V>\<^sub>1) (C', \<V>\<^sub>3)"
     proof(rule superpositionI)
       show "term_subst.is_renaming \<rho>\<^sub>1"
-        using renaming(1).
+        using \<rho>\<^sub>1.
     next
       show "term_subst.is_renaming \<rho>\<^sub>2"
-        using renaming(2).
+        using \<rho>\<^sub>2.
     next 
-      show "premise\<^sub>1 = add_mset literal\<^sub>1 premise\<^sub>1'"
-        using premise\<^sub>1.
+      show "E = add_mset l\<^sub>1 E'"
+        using E.
     next
-      show "premise\<^sub>2 = add_mset literal\<^sub>2 premise\<^sub>2'"
-        using premise\<^sub>2.
+      show "D = add_mset l\<^sub>2 D'"
+        using D.
     next
       show "?\<P> \<in> {Pos, Neg}"
         by simp
     next
-      show "literal\<^sub>1 = ?\<P> (Upair context\<^sub>1\<langle>term\<^sub>1\<rangle> term\<^sub>1')"
-        unfolding literal\<^sub>1 term\<^sub>1_with_context..
+      show "l\<^sub>1 = ?\<P> (Upair c\<^sub>1\<langle>t\<^sub>1\<rangle> t\<^sub>1')"
+        unfolding l\<^sub>1 ..
     next
-      show "literal\<^sub>2 = term\<^sub>2 \<approx> term\<^sub>2'"
-        using literal\<^sub>2.
+      show "l\<^sub>2 = t\<^sub>2 \<approx> t\<^sub>2'"
+        using l\<^sub>2.
     next
-      show "is_Fun term\<^sub>1"
-        using term\<^sub>1_not_Var.
+      show "is_Fun t\<^sub>1"
+        using t\<^sub>1_is_Fun.
     next
-      show "term_subst.is_imgu \<mu> {{term\<^sub>1 \<cdot>t \<rho>\<^sub>1, term\<^sub>2 \<cdot>t \<rho>\<^sub>2}}"
+      show "term_subst.is_imgu \<mu> {{t\<^sub>1 \<cdot>t \<rho>\<^sub>1, t\<^sub>2 \<cdot>t \<rho>\<^sub>2}}"
         using \<mu>(1).
     next
-      note premises_clause_to_ground_inverse = assms(9, 10)[THEN clause.to_ground_inverse]  
-      note premise_groundings = assms(10, 9)[unfolded \<mu>(2) clause.subst_comp_subst]
+      note premises_clause_to_ground_inverse = assms(10, 11)[THEN clause.to_ground_inverse]  
+      note N\<^sub>G = assms(11, 10)[unfolded \<mu>(2) clause.subst_comp_subst]
 
-      have "premise\<^sub>2 \<cdot> \<rho>\<^sub>2 \<cdot> \<mu> \<cdot> \<sigma> \<prec>\<^sub>c premise\<^sub>1 \<cdot> \<rho>\<^sub>1 \<cdot> \<mu> \<cdot> \<sigma>"
+      have "D \<cdot> \<rho>\<^sub>2 \<cdot> \<mu> \<cdot> \<sigma> \<prec>\<^sub>c E \<cdot> \<rho>\<^sub>1 \<cdot> \<mu> \<cdot> \<sigma>"
         using ground_superpositionI(3) 
-        unfolding premise\<^sub>G\<^sub>1 premise\<^sub>G\<^sub>2 clause.order.less\<^sub>G_def premises_clause_to_ground_inverse 
+        unfolding E\<^sub>G D\<^sub>G clause.order.less\<^sub>G_def premises_clause_to_ground_inverse 
         unfolding \<mu>(2) clause.subst_comp_subst 
         by blast
 
-      then show "\<not> premise\<^sub>1 \<cdot> \<rho>\<^sub>1 \<cdot> \<mu> \<preceq>\<^sub>c premise\<^sub>2 \<cdot> \<rho>\<^sub>2 \<cdot> \<mu>"
-        using clause.order.ground_less_not_less_eq[OF premise_groundings]
+      then show "\<not> E \<cdot> \<rho>\<^sub>1 \<cdot> \<mu> \<preceq>\<^sub>c D \<cdot> \<rho>\<^sub>2 \<cdot> \<mu>"
+        using clause.order.ground_less_not_less_eq[OF N\<^sub>G]
         by blast
     next
       show "?\<P> = Pos 
-              \<and> select premise\<^sub>1 = {#} 
-              \<and> is_strictly_maximal (literal\<^sub>1 \<cdot>l \<rho>\<^sub>1 \<cdot>l \<mu>) (premise\<^sub>1 \<cdot> \<rho>\<^sub>1 \<cdot> \<mu>) 
+              \<and> select E = {#} 
+              \<and> is_strictly_maximal (l\<^sub>1 \<cdot>l \<rho>\<^sub>1 \<cdot>l \<mu>) (E \<cdot> \<rho>\<^sub>1 \<cdot> \<mu>) 
           \<or> ?\<P> = Neg 
-              \<and> (select premise\<^sub>1 = {#} \<and> is_maximal (literal\<^sub>1 \<cdot>l \<rho>\<^sub>1 \<cdot>l \<mu>) (premise\<^sub>1 \<cdot> \<rho>\<^sub>1 \<cdot> \<mu>) 
-                 \<or> is_maximal (literal\<^sub>1 \<cdot>l \<rho>\<^sub>1 \<cdot>l \<mu>) ((select premise\<^sub>1) \<cdot> \<rho>\<^sub>1 \<cdot> \<mu>))"
+              \<and> (select E = {#} \<and> is_maximal (l\<^sub>1 \<cdot>l \<rho>\<^sub>1 \<cdot>l \<mu>) (E \<cdot> \<rho>\<^sub>1 \<cdot> \<mu>) 
+                 \<or> is_maximal (l\<^sub>1 \<cdot>l \<rho>\<^sub>1 \<cdot>l \<mu>) ((select E) \<cdot> \<rho>\<^sub>1 \<cdot> \<mu>))"
       proof(cases "?\<P> = Pos")
         case True
-        moreover then have select_empty: "select premise\<^sub>1 = {#}"
-          using clause_subst_empty select(1) ground_superpositionI(9) 
-          by auto
+        moreover then have select_empty: "select E = {#}"
+          using clause_subst_empty(2) select_from_E ground_superpositionI(9) 
+          by (metis clause_from_ground_empty_mset literals_distinct(1))
 
-        moreover have "is_strictly_maximal (literal\<^sub>1 \<cdot>l \<rho>\<^sub>1 \<cdot>l \<mu> \<cdot>l \<sigma>) (premise\<^sub>1 \<cdot> \<rho>\<^sub>1 \<cdot> \<mu> \<cdot> \<sigma>)"
-          using True pos_literal\<^sub>G\<^sub>1_is_strictly_maximal\<^sub>l
-          unfolding literal\<^sub>1_\<gamma>[symmetric] \<mu>(2)
-          by force
+        moreover have "is_strictly_maximal (l\<^sub>1 \<cdot>l \<rho>\<^sub>1 \<cdot>l \<mu> \<cdot>l \<sigma>) (E \<cdot> \<rho>\<^sub>1 \<cdot> \<mu> \<cdot> \<sigma>)"
+          using True l\<^sub>1_\<gamma> \<mu>(2)
+          by (smt (verit, ccfv_SIG) E_\<gamma> clause.subst_comp_subst clause_safe_unfolds(4,6) ground_superpositionI(1,5,9)
+              literal.comp_subst.left.monoid_action_compatibility literals_distinct
+              nonground_context.term_from_ground_context_from_ground)
 
-        moreover then have "is_strictly_maximal (literal\<^sub>1 \<cdot>l \<rho>\<^sub>1 \<cdot>l \<mu>) (premise\<^sub>1 \<cdot> \<rho>\<^sub>1 \<cdot> \<mu>)"
+        moreover then have "is_strictly_maximal (l\<^sub>1 \<cdot>l \<rho>\<^sub>1 \<cdot>l \<mu>) (E \<cdot> \<rho>\<^sub>1 \<cdot> \<mu>)"
           using 
             is_strictly_maximal_if_grounding_is_strictly_maximal[OF
               _
-              premise\<^sub>1_grounding[unfolded \<mu>(2) clause.subst_comp_subst]
+              E_grounding[unfolded \<mu>(2)]
               ]
             clause.subst_in_to_set_subst
-            literal\<^sub>1_in_premise\<^sub>1
-          by blast
+            l\<^sub>1_in_E
+          by (metis (no_types, lifting) \<mu>(2) assms(10) clause.subst_comp_subst
+              is_strictly_maximal_if_grounding_is_strictly_maximal)
 
         ultimately show ?thesis
           by auto
@@ -1382,149 +1232,145 @@ proof(cases premise\<^sub>G\<^sub>2 premise\<^sub>G\<^sub>1 conclusion\<^sub>G r
         proof(cases ?select\<^sub>G_empty)
           case select\<^sub>G_empty: True
 
-          then have "select premise\<^sub>1 = {#}"
-            using clause_subst_empty select(1) ground_superpositionI(9) \<P>\<^sub>G_Neg
+          then have "select E = {#}"
+            using clause_subst_empty select_from_E ground_superpositionI(9) \<P>\<^sub>G_Neg
             by simp
 
-          moreover have "is_maximal (literal\<^sub>1 \<cdot>l \<rho>\<^sub>1 \<cdot>l \<mu> \<cdot>l \<sigma>) (premise\<^sub>1 \<cdot> \<rho>\<^sub>1 \<cdot> \<mu> \<cdot> \<sigma>)"
-            using neg_literal\<^sub>G\<^sub>1_is_maximal\<^sub>l[OF select\<^sub>G_empty]
-            unfolding literal\<^sub>1_\<gamma>[symmetric] \<mu>(2)
-            by simp
+          moreover have "is_maximal (l\<^sub>1 \<cdot>l \<rho>\<^sub>1 \<cdot>l \<mu> \<cdot>l \<sigma>) (E \<cdot> \<rho>\<^sub>1 \<cdot> \<mu> \<cdot> \<sigma>)"
+            using l\<^sub>1_\<gamma> \<mu>(2)
+            using E_\<gamma> ground_superpositionI(5,9) is_maximal_empty select\<^sub>G_empty by auto
 
-          moreover then have "is_maximal (literal\<^sub>1 \<cdot>l \<rho>\<^sub>1 \<cdot>l \<mu>) (premise\<^sub>1 \<cdot> \<rho>\<^sub>1 \<cdot> \<mu>)"
+          moreover then have "is_maximal (l\<^sub>1 \<cdot>l \<rho>\<^sub>1 \<cdot>l \<mu>) (E \<cdot> \<rho>\<^sub>1 \<cdot> \<mu>)"
             using 
               is_maximal_if_grounding_is_maximal[OF 
                 _  
-                premise\<^sub>1_grounding[unfolded \<mu>(2) clause.subst_comp_subst]
+                E_grounding[unfolded \<mu>(2)]
                 ]
               clause.subst_in_to_set_subst
-              literal\<^sub>1_in_premise\<^sub>1
-            by blast
+              l\<^sub>1_in_E
+            by (metis (no_types, lifting) \<mu>(2) assms(10) clause.subst_comp_subst is_maximal_if_grounding_is_maximal)
 
           ultimately show ?thesis
             using \<P>\<^sub>G_Neg
-            by simp
+            by auto
         next
           case select\<^sub>G_not_empty: False
 
-          have selected_grounding: "clause.is_ground (select premise\<^sub>1 \<cdot> \<rho>\<^sub>1 \<cdot> \<mu> \<cdot> \<sigma>)"
-            using select_ground_subst[OF premise\<^sub>1_grounding] select(1)
+          have selected_grounding: "clause.is_ground (select E \<cdot> \<rho>\<^sub>1 \<cdot> \<mu> \<cdot> \<sigma>)"
+            using select_ground_subst[OF E_grounding] select_from_E
             unfolding \<mu>(2) clause.subst_comp_subst
             by (metis clause.ground_is_ground)
 
           note selected_subst =
-            literal\<^sub>1_selected[
+            l\<^sub>1_selected[
               OF \<P>\<^sub>G_Neg select\<^sub>G_not_empty, 
               THEN maximal_in_clause, 
               THEN clause.subst_in_to_set_subst] 
 
-          have "is_maximal (literal\<^sub>1  \<cdot>l \<rho>\<^sub>1 \<cdot>l \<gamma>) (select premise\<^sub>1 \<cdot> \<rho>\<^sub>1 \<cdot> \<gamma>)"  
+          have "is_maximal (l\<^sub>1 \<cdot>l \<rho>\<^sub>1 \<cdot>l \<gamma>) (select E \<cdot> \<rho>\<^sub>1 \<cdot> \<gamma>)"  
             using select\<^sub>G_not_empty ground_superpositionI(9) \<P>\<^sub>G_Neg 
-            unfolding literal\<^sub>1_\<gamma>[symmetric] select(1)
-            by simp
+            using l\<^sub>1_\<gamma> select_from_E
+            using E\<^sub>G \<open>(\<P>\<^sub>G \<noteq> Pos) = (\<P>\<^sub>G = Neg)\<close> ground_superpositionI(5) 
+            by fastforce
 
-          then have "is_maximal (literal\<^sub>1 \<cdot>l \<rho>\<^sub>1 \<cdot>l \<mu>) ((select premise\<^sub>1) \<cdot> \<rho>\<^sub>1 \<cdot> \<mu>)"
+          then have "is_maximal (l\<^sub>1 \<cdot>l \<rho>\<^sub>1 \<cdot>l \<mu>) ((select E) \<cdot> \<rho>\<^sub>1 \<cdot> \<mu>)"
             using is_maximal_if_grounding_is_maximal[OF _ selected_grounding] selected_subst
             by (metis \<mu>(2) clause.subst_comp_subst literal.subst_comp_subst)
 
           with select\<^sub>G_not_empty \<P>\<^sub>G_Neg show ?thesis
-            by simp
+            by auto
         qed
       qed
     next
-      show "select premise\<^sub>2 = {#}"
-        using ground_superpositionI(10) select(2)
+      show "select D = {#}"
+        using ground_superpositionI(10) select_from_D
         by simp
     next 
-      have "is_strictly_maximal (literal\<^sub>2 \<cdot>l \<rho>\<^sub>2 \<cdot>l \<mu> \<cdot>l \<sigma>) (premise\<^sub>2 \<cdot> \<rho>\<^sub>2 \<cdot> \<mu> \<cdot> \<sigma>)"
-        using literal\<^sub>G\<^sub>2_is_strictly_maximal\<^sub>l
-        unfolding literal\<^sub>2_\<gamma>[symmetric] \<mu>(2)
-        by simp
+      have "is_strictly_maximal (l\<^sub>2 \<cdot>l \<rho>\<^sub>2 \<cdot>l \<mu> \<cdot>l \<sigma>) (D \<cdot> \<rho>\<^sub>2 \<cdot> \<mu> \<cdot> \<sigma>)"
+        using l\<^sub>2_\<gamma> \<mu>(2)
+        using D_\<gamma> ground_superpositionI(11,6) by auto
 
-      then show "is_strictly_maximal (literal\<^sub>2 \<cdot>l \<rho>\<^sub>2 \<cdot>l \<mu>) (premise\<^sub>2 \<cdot> \<rho>\<^sub>2 \<cdot> \<mu>)"
+      then show "is_strictly_maximal (l\<^sub>2 \<cdot>l \<rho>\<^sub>2 \<cdot>l \<mu>) (D \<cdot> \<rho>\<^sub>2 \<cdot> \<mu>)"
         using 
           is_strictly_maximal_if_grounding_is_strictly_maximal[OF 
-            _  premise\<^sub>2_grounding[unfolded \<mu>(2) clause.subst_comp_subst]]
-          literal\<^sub>2_in_premise\<^sub>2
+            _  D_grounding[unfolded \<mu>(2) clause.subst_comp_subst]]
+          l\<^sub>2_in_D
           clause.subst_in_to_set_subst
         by blast
     next
       have term_groundings: 
-        "term.is_ground (term\<^sub>1' \<cdot>t \<rho>\<^sub>1 \<cdot>t \<mu> \<cdot>t \<sigma>)" 
-        "term.is_ground (context\<^sub>1\<langle>term\<^sub>1\<rangle> \<cdot>t \<rho>\<^sub>1 \<cdot>t \<mu> \<cdot>t \<sigma>)" 
-        unfolding 
-          term\<^sub>1_with_context[symmetric]  
-          term\<^sub>1_with_context_\<gamma>[unfolded \<mu>(2) term_subst.subst_comp_subst]
-          term\<^sub>1'_\<gamma>[unfolded \<mu>(2) term_subst.subst_comp_subst]
+        "term.is_ground (t\<^sub>1' \<cdot>t \<rho>\<^sub>1 \<cdot>t \<mu> \<cdot>t \<sigma>)" 
+        "term.is_ground (c\<^sub>1\<langle>t\<^sub>1\<rangle> \<cdot>t \<rho>\<^sub>1 \<cdot>t \<mu> \<cdot>t \<sigma>)" 
+        using t\<^sub>1'_\<gamma> \<mu>(2) t\<^sub>1_\<gamma> c\<^sub>1_\<gamma>
         by simp_all
 
-      have "term\<^sub>1' \<cdot>t \<rho>\<^sub>1 \<cdot>t \<mu> \<cdot>t \<sigma> \<prec>\<^sub>t context\<^sub>1\<langle>term\<^sub>1\<rangle> \<cdot>t \<rho>\<^sub>1 \<cdot>t \<mu> \<cdot>t \<sigma>"
-        using ground_superpositionI(7) 
+      have "t\<^sub>1' \<cdot>t \<rho>\<^sub>1 \<cdot>t \<mu> \<cdot>t \<sigma> \<prec>\<^sub>t c\<^sub>1\<langle>t\<^sub>1\<rangle> \<cdot>t \<rho>\<^sub>1 \<cdot>t \<mu> \<cdot>t \<sigma>"
+        using ground_superpositionI(7) c\<^sub>1_\<gamma>[unfolded \<mu>(2)]
         unfolding 
-          term\<^sub>1'_\<gamma>[unfolded \<mu>(2) term_subst.subst_comp_subst]
-          term\<^sub>1_with_context[symmetric]
-          term\<^sub>1_with_context_\<gamma>[unfolded \<mu>(2) term_subst.subst_comp_subst]
+          t\<^sub>1'_\<gamma>[unfolded \<mu>(2) term_subst.subst_comp_subst]
+          t\<^sub>1_\<gamma>[unfolded \<mu>(2) term_subst.subst_comp_subst]
           term.order.less\<^sub>G_def
-          context.safe_unfolds.
+          context.safe_unfolds
+        by simp
 
-      then show "\<not> context\<^sub>1\<langle>term\<^sub>1\<rangle> \<cdot>t \<rho>\<^sub>1 \<cdot>t \<mu> \<preceq>\<^sub>t term\<^sub>1' \<cdot>t \<rho>\<^sub>1 \<cdot>t \<mu>"
+      then show "\<not> c\<^sub>1\<langle>t\<^sub>1\<rangle> \<cdot>t \<rho>\<^sub>1 \<cdot>t \<mu> \<preceq>\<^sub>t t\<^sub>1' \<cdot>t \<rho>\<^sub>1 \<cdot>t \<mu>"
         using term.order.ground_less_not_less_eq[OF term_groundings]
         by blast
     next
       have term_groundings: 
-        "term.is_ground (term\<^sub>2' \<cdot>t \<rho>\<^sub>2 \<cdot>t \<mu> \<cdot>t \<sigma>)"
-        "term.is_ground (term\<^sub>2 \<cdot>t \<rho>\<^sub>2 \<cdot>t \<mu> \<cdot>t \<sigma>)"
+        "term.is_ground (t\<^sub>2' \<cdot>t \<rho>\<^sub>2 \<cdot>t \<mu> \<cdot>t \<sigma>)"
+        "term.is_ground (t\<^sub>2 \<cdot>t \<rho>\<^sub>2 \<cdot>t \<mu> \<cdot>t \<sigma>)"
         unfolding
-          term\<^sub>2_\<gamma>[unfolded \<mu>(2) term_subst.subst_comp_subst]
-          term\<^sub>2'_\<gamma>[unfolded \<mu>(2) term_subst.subst_comp_subst]
+          t\<^sub>2_\<gamma>[unfolded \<mu>(2) term_subst.subst_comp_subst]
+          t\<^sub>2'_\<gamma>[unfolded \<mu>(2) term_subst.subst_comp_subst]
         by simp_all
 
-      have "term\<^sub>2' \<cdot>t \<rho>\<^sub>2 \<cdot>t \<mu> \<cdot>t \<sigma> \<prec>\<^sub>t term\<^sub>2 \<cdot>t \<rho>\<^sub>2 \<cdot>t \<mu> \<cdot>t \<sigma>"
+      have "t\<^sub>2' \<cdot>t \<rho>\<^sub>2 \<cdot>t \<mu> \<cdot>t \<sigma> \<prec>\<^sub>t t\<^sub>2 \<cdot>t \<rho>\<^sub>2 \<cdot>t \<mu> \<cdot>t \<sigma>"
         using ground_superpositionI(8)
         unfolding
-          term\<^sub>2_\<gamma>[unfolded \<mu>(2) term_subst.subst_comp_subst]       
-          term\<^sub>2'_\<gamma>[unfolded \<mu>(2) term_subst.subst_comp_subst]
+          t\<^sub>2_\<gamma>[unfolded \<mu>(2) term_subst.subst_comp_subst]       
+          t\<^sub>2'_\<gamma>[unfolded \<mu>(2) term_subst.subst_comp_subst]
           term.order.less\<^sub>G_def.
 
-      then show "\<not> term\<^sub>2 \<cdot>t \<rho>\<^sub>2 \<cdot>t \<mu> \<preceq>\<^sub>t term\<^sub>2' \<cdot>t \<rho>\<^sub>2 \<cdot>t \<mu>"
+      then show "\<not> t\<^sub>2 \<cdot>t \<rho>\<^sub>2 \<cdot>t \<mu> \<preceq>\<^sub>t t\<^sub>2' \<cdot>t \<rho>\<^sub>2 \<cdot>t \<mu>"
         using term.order.ground_less_not_less_eq[OF term_groundings]
         by blast
     next
       show 
-        "conclusion' = add_mset (?\<P> (Upair (context\<^sub>1 \<cdot>t\<^sub>c \<rho>\<^sub>1)\<langle>term\<^sub>2' \<cdot>t \<rho>\<^sub>2\<rangle> (term\<^sub>1' \<cdot>t \<rho>\<^sub>1))) 
-          (premise\<^sub>1' \<cdot> \<rho>\<^sub>1 + premise\<^sub>2' \<cdot> \<rho>\<^sub>2) \<cdot> \<mu>"
-        unfolding term\<^sub>2'_with_context conclusion'..
-      show "welltyped_imgu \<V>\<^sub>3 (term\<^sub>1 \<cdot>t \<rho>\<^sub>1) (term\<^sub>2 \<cdot>t \<rho>\<^sub>2) \<mu>"
+        "C' = add_mset (?\<P> (Upair (c\<^sub>1 \<cdot>t\<^sub>c \<rho>\<^sub>1)\<langle>t\<^sub>2' \<cdot>t \<rho>\<^sub>2\<rangle> (t\<^sub>1' \<cdot>t \<rho>\<^sub>1))) 
+          (E' \<cdot> \<rho>\<^sub>1 + D' \<cdot> \<rho>\<^sub>2) \<cdot> \<mu>"
+        unfolding  C'..
+      show "welltyped_imgu \<V>\<^sub>3 (t\<^sub>1 \<cdot>t \<rho>\<^sub>1) (t\<^sub>2 \<cdot>t \<rho>\<^sub>2) \<mu>"
         using \<mu>(3) by blast
 
-      show "clause.vars (premise\<^sub>1 \<cdot> \<rho>\<^sub>1) \<inter> clause.vars (premise\<^sub>2 \<cdot> \<rho>\<^sub>2) = {}"
-        using renaming(3). 
+      show "clause.vars (E \<cdot> \<rho>\<^sub>1) \<inter> clause.vars (D \<cdot> \<rho>\<^sub>2) = {}"
+        using rename_apart. 
 
-      show "\<forall>x\<in>clause.vars (premise\<^sub>1 \<cdot> \<rho>\<^sub>1). \<V>\<^sub>1 (inv \<rho>\<^sub>1 (Var x)) = \<V>\<^sub>3 x"
+      show "\<forall>x\<in>clause.vars (E \<cdot> \<rho>\<^sub>1). \<V>\<^sub>1 (inv \<rho>\<^sub>1 (Var x)) = \<V>\<^sub>3 x"
         unfolding \<V>\<^sub>3_def
         by meson
 
-      show "\<forall>x\<in>clause.vars (premise\<^sub>2 \<cdot> \<rho>\<^sub>2). \<V>\<^sub>2 (inv \<rho>\<^sub>2 (Var x)) = \<V>\<^sub>3 x"
+      show "\<forall>x\<in>clause.vars (D \<cdot> \<rho>\<^sub>2). \<V>\<^sub>2 (inv \<rho>\<^sub>2 (Var x)) = \<V>\<^sub>3 x"
         unfolding \<V>\<^sub>3_def
-        using renaming(3)
+        using rename_apart
         by (meson disjoint_iff)
 
-      show "is_welltyped_on (clause.vars premise\<^sub>1) \<V>\<^sub>1 \<rho>\<^sub>1"
-        using typing(5).
+      show "is_welltyped_on (clause.vars E) \<V>\<^sub>1 \<rho>\<^sub>1"
+        using \<rho>\<^sub>1_is_welltyped.
 
-      show "is_welltyped_on (clause.vars premise\<^sub>2) \<V>\<^sub>2 \<rho>\<^sub>2"
-        using typing(6).
+      show "is_welltyped_on (clause.vars D) \<V>\<^sub>2 \<rho>\<^sub>2"
+        using \<rho>\<^sub>2_is_welltyped.
 
-      have "\<exists>\<tau>. welltyped \<V>\<^sub>2 term\<^sub>2 \<tau> \<and> welltyped \<V>\<^sub>2 term\<^sub>2' \<tau>"
-        using typing(2)
-        unfolding premise\<^sub>2 literal\<^sub>2
+      have "\<exists>\<tau>. welltyped \<V>\<^sub>2 t\<^sub>2 \<tau> \<and> welltyped \<V>\<^sub>2 t\<^sub>2' \<tau>"
+        using D_is_welltyped
+        unfolding D l\<^sub>2
         by auto
 
-      then show "\<And>\<tau> \<tau>'. \<lbrakk>typed \<V>\<^sub>2 term\<^sub>2 \<tau>; typed \<V>\<^sub>2 term\<^sub>2' \<tau>'\<rbrakk> \<Longrightarrow> \<tau> = \<tau>'"
+      then show "\<And>\<tau> \<tau>'. \<lbrakk>typed \<V>\<^sub>2 t\<^sub>2 \<tau>; typed \<V>\<^sub>2 t\<^sub>2' \<tau>'\<rbrakk> \<Longrightarrow> \<tau> = \<tau>'"
         using term.typed_if_welltyped by blast
 
       show "infinite_variables_per_type \<V>\<^sub>1" "infinite_variables_per_type \<V>\<^sub>2"
-        using typing
+        using \<V>\<^sub>1 \<V>\<^sub>2
         by auto
     qed
 
@@ -1536,127 +1382,116 @@ proof(cases premise\<^sub>G\<^sub>2 premise\<^sub>G\<^sub>1 conclusion\<^sub>G r
       unfolding \<mu>(2) term_subst.is_idem_def
       by (metis subst_compose_assoc)
 
-    have conclusion'_\<gamma>: "conclusion' \<cdot> \<gamma> = conclusion \<cdot> \<gamma>"
+    have C'_\<gamma>: "C' \<cdot> \<gamma> = C \<cdot> \<gamma>"
     proof-
-      have "conclusion \<cdot> \<gamma> = 
-              add_mset (?\<P> (Upair (context.from_ground context\<^sub>G)\<langle>term.from_ground term\<^sub>G\<^sub>3\<rangle> (term.from_ground term\<^sub>G\<^sub>2))) 
-                (clause.from_ground premise\<^sub>G\<^sub>1' + clause.from_ground premise\<^sub>G\<^sub>2')"
-        using ground_superpositionI(4, 12) clause.to_ground_inverse[OF conclusion_grounding] 
+      have "C \<cdot> \<gamma> = 
+              add_mset (?\<P> (Upair (context.from_ground c\<^sub>G)\<langle>term.from_ground t\<^sub>G\<^sub>3\<rangle> (term.from_ground t\<^sub>G\<^sub>2))) 
+                (clause.from_ground E\<^sub>G' + clause.from_ground D\<^sub>G')"
+        using ground_superpositionI(4, 12) clause.to_ground_inverse[OF C_grounding] 
         by auto
-      
+
       then show ?thesis
         unfolding 
-          conclusion'
-          term\<^sub>2'_with_context_\<gamma>[symmetric]
-          premise\<^sub>1'_\<gamma>[symmetric] 
-          premise\<^sub>2'_\<gamma>[symmetric] 
-          term\<^sub>1'_\<gamma>[symmetric]
-          clause.plus_subst[symmetric] 
-          subst_apply_term_ctxt_apply_distrib[symmetric]
-          subst_atom[symmetric]
+          C'
+          E'_\<gamma>[symmetric] 
+          D'_\<gamma>[symmetric] 
+          t\<^sub>1'_\<gamma>[symmetric]
+          c\<^sub>1_t\<^sub>2'_\<gamma>[symmetric]
         unfolding
           clause.subst_comp_subst[symmetric]
           \<mu>_\<gamma>
         by simp
     qed
 
-    have vars_conclusion': 
-      "clause.vars conclusion' \<subseteq> clause.vars (premise\<^sub>1 \<cdot> \<rho>\<^sub>1) \<union> clause.vars (premise\<^sub>2 \<cdot> \<rho>\<^sub>2)"
+    have vars_C': 
+      "clause.vars C' \<subseteq> clause.vars (E \<cdot> \<rho>\<^sub>1) \<union> clause.vars (D \<cdot> \<rho>\<^sub>2)"
     proof
       fix x 
-      assume "x \<in> clause.vars conclusion'"
+      assume "x \<in> clause.vars C'"
 
       then consider 
-          (term\<^sub>2'_with_context) "x \<in> term.vars (term\<^sub>2'_with_context \<cdot>t \<mu>)" 
-        | (term\<^sub>1')  "x \<in> term.vars (term\<^sub>1' \<cdot>t \<rho>\<^sub>1 \<cdot>t \<mu>)"  
-        | (premise\<^sub>1')  "x \<in> clause.vars (premise\<^sub>1' \<cdot> \<rho>\<^sub>1 \<cdot> \<mu>)"  
-        | (premise\<^sub>2')  "x \<in> clause.vars (premise\<^sub>2' \<cdot> \<rho>\<^sub>2 \<cdot> \<mu>)"  
-        unfolding conclusion' clause.add_subst clause.plus_subst subst_literal
+        (term\<^sub>2'_with_context) "x \<in> term.vars ((c\<^sub>1 \<cdot>t\<^sub>c \<rho>\<^sub>1)\<langle>t\<^sub>2' \<cdot>t \<rho>\<^sub>2\<rangle> \<cdot>t \<mu>)" 
+        | (term\<^sub>1')  "x \<in> term.vars (t\<^sub>1' \<cdot>t \<rho>\<^sub>1 \<cdot>t \<mu>)"  
+        | (E')  "x \<in> clause.vars (E' \<cdot> \<rho>\<^sub>1 \<cdot> \<mu>)"  
+        | (D')  "x \<in> clause.vars (D' \<cdot> \<rho>\<^sub>2 \<cdot> \<mu>)"  
+        unfolding C' clause.add_subst clause.plus_subst subst_literal
         by auto
-  
-      then show "x \<in> clause.vars (premise\<^sub>1 \<cdot> \<rho>\<^sub>1) \<union> clause.vars (premise\<^sub>2 \<cdot> \<rho>\<^sub>2)"
+
+      then show "x \<in> clause.vars (E \<cdot> \<rho>\<^sub>1) \<union> clause.vars (D \<cdot> \<rho>\<^sub>2)"
       proof(cases)
         case t: term\<^sub>2'_with_context
         then show ?thesis 
           using  context.variables_in_base_imgu[OF \<mu>(1)] term.variables_in_base_imgu[OF \<mu>(1)] 
-          unfolding premise\<^sub>1 literal\<^sub>1 term\<^sub>1_with_context premise\<^sub>2 literal\<^sub>2  term\<^sub>2'_with_context
-          (* TODO: *)
+          unfolding E l\<^sub>1 D l\<^sub>2
+            (* TODO: *)
           apply auto
-          by (smt (verit, ccfv_threshold) UnE in_mono t term\<^sub>2'_with_context
-              vars_term_ctxt_apply)
+          by (smt (verit, ccfv_threshold) UnE in_mono t vars_term_ctxt_apply)
       next
         case term\<^sub>1'
         then show ?thesis
           using term.variables_in_base_imgu[OF \<mu>(1)]
-          unfolding premise\<^sub>1 clause.add_subst literal\<^sub>1 term\<^sub>1_with_context premise\<^sub>2 literal\<^sub>2
+          unfolding E clause.add_subst l\<^sub>1 D l\<^sub>2
           by auto
       next
-        case premise\<^sub>1'
+        case E'
         then show ?thesis 
           using clause.variables_in_base_imgu[OF \<mu>(1)]
-          unfolding premise\<^sub>1 clause.add_subst literal\<^sub>1 term\<^sub>1_with_context premise\<^sub>2 literal\<^sub>2
+          unfolding E l\<^sub>1 D l\<^sub>2
           by auto
-       next
-        case premise\<^sub>2'
+      next
+        case D'
         then show ?thesis 
           using clause.variables_in_base_imgu[OF \<mu>(1)]
-          unfolding premise\<^sub>1 clause.add_subst literal\<^sub>1 term\<^sub>1_with_context premise\<^sub>2 literal\<^sub>2
+          unfolding E l\<^sub>1 D l\<^sub>2
           by auto
       qed
     qed
 
     have surjx: "surj (\<lambda>x. inv \<rho>\<^sub>2 (Var x))"
-      using term.surj_inv_renaming[OF renaming(2)].
-                  
-    have yy: 
-      "\<And>P Q b ty. {x. (if b x then P x else Q x) = ty } = 
-        {x. b x \<and> P x = ty} \<union> {x. \<not>b x \<and> Q x = ty}"
-      by auto
+      using term.surj_inv_renaming[OF \<rho>\<^sub>2].
 
-    have qq: "\<And>ty. infinite {x. \<V>\<^sub>2 (inv \<rho>\<^sub>2 (Var x)) = ty}"
-      using surj_infinite_set[OF surjx typing(8)[unfolded infinite_variables_per_type_def, rule_format]].
+    have infinite_variables_per_type_\<V>\<^sub>3: "infinite_variables_per_type \<V>\<^sub>3"
+    proof(unfold infinite_variables_per_type_def \<V>\<^sub>3_def if_distrib if_distribR move_simp Finite_Set.infinite_Un zz, intro allI disjI2 Diff_infinite_finite)
+      fix ty
+      show "finite {x. x \<in> clause.vars (E \<cdot> \<rho>\<^sub>1)}"
+        using clause.finite_vars[of "E \<cdot> \<rho>\<^sub>1"]
+        by simp
 
-    have zz: 
-      "\<And>ty. {x. x \<notin> clause.vars (premise\<^sub>1 \<cdot> \<rho>\<^sub>1) \<and> \<V>\<^sub>2 (inv \<rho>\<^sub>2 (Var x)) = ty} = 
-            {x. \<V>\<^sub>2 (inv \<rho>\<^sub>2 (Var x)) = ty} - {x. x \<in> clause.vars (premise\<^sub>1 \<cdot> \<rho>\<^sub>1)}"
-      by auto
+      show "infinite {x. \<V>\<^sub>2 (inv \<rho>\<^sub>2 (Var x)) = ty}"
+        using 
+          surj_infinite_set[OF 
+            surjx \<V>\<^sub>2[unfolded infinite_variables_per_type_def, rule_format]].
+    qed
 
-    have "\<And>ty. infinite {x. x \<notin> clause.vars (premise\<^sub>1 \<cdot> \<rho>\<^sub>1) \<and> \<V>\<^sub>2 (inv \<rho>\<^sub>2 (Var x)) = ty}"
-      unfolding zz
-      using qq clause.finite_vars[of "premise\<^sub>1 \<cdot> \<rho>\<^sub>1"]
-      by simp
-
-    then have infinite_variables_per_type_\<V>\<^sub>3: "infinite_variables_per_type \<V>\<^sub>3"   
-      unfolding \<V>\<^sub>3_def infinite_variables_per_type_def yy     
-      by auto
-
-    show "\<iota>\<^sub>G \<in> inference_groundings (Infer [(premise\<^sub>2, \<V>\<^sub>2), (premise\<^sub>1, \<V>\<^sub>1)] (conclusion', \<V>\<^sub>3))"
+    show "\<iota>\<^sub>G \<in> inference_groundings (Infer [(D, \<V>\<^sub>2), (E, \<V>\<^sub>1)] (C', \<V>\<^sub>3))"
     proof-
-      have " \<lbrakk>conclusion' \<cdot> \<gamma> = conclusion \<cdot> \<gamma>;
-         ground.superposition (clause.to_ground (premise\<^sub>2 \<cdot> \<rho>\<^sub>2 \<cdot> \<gamma>))
-          (clause.to_ground (premise\<^sub>1 \<cdot> \<rho>\<^sub>1 \<cdot> \<gamma>)) (clause.to_ground (conclusion \<cdot> \<gamma>));
-         is_welltyped_on (clause.vars conclusion') \<V>\<^sub>3 \<gamma>; infinite_variables_per_type \<V>\<^sub>3\<rbrakk>
-        \<Longrightarrow> clause.is_welltyped \<V>\<^sub>3 conclusion'"
-        using \<open>superposition (premise\<^sub>2, \<V>\<^sub>2) (premise\<^sub>1, \<V>\<^sub>1) (conclusion', \<V>\<^sub>3)\<close> 
-          superposition_preserves_typing typing(1) typing(2) by blast
+      have " \<lbrakk>C' \<cdot> \<gamma> = C \<cdot> \<gamma>;
+         ground.superposition (clause.to_ground (D \<cdot> \<rho>\<^sub>2 \<cdot> \<gamma>))
+          (clause.to_ground (E \<cdot> \<rho>\<^sub>1 \<cdot> \<gamma>)) (clause.to_ground (C \<cdot> \<gamma>));
+         is_welltyped_on (clause.vars C') \<V>\<^sub>3 \<gamma>; infinite_variables_per_type \<V>\<^sub>3\<rbrakk>
+        \<Longrightarrow> clause.is_welltyped \<V>\<^sub>3 C'"
+        using \<open>superposition (D, \<V>\<^sub>2) (E, \<V>\<^sub>1) (C', \<V>\<^sub>3)\<close> 
+          superposition_preserves_typing E_is_welltyped D_is_welltyped by blast
 
       then have 
-        "is_inference_grounding (Infer [(premise\<^sub>2, \<V>\<^sub>2), (premise\<^sub>1, \<V>\<^sub>1)] (conclusion', \<V>\<^sub>3)) \<iota>\<^sub>G \<gamma> \<rho>\<^sub>1 \<rho>\<^sub>2"
+        "is_inference_grounding (Infer [(D, \<V>\<^sub>2), (E, \<V>\<^sub>1)] (C', \<V>\<^sub>3)) \<iota>\<^sub>G \<gamma> \<rho>\<^sub>1 \<rho>\<^sub>2"
         using 
-          conclusion'_\<gamma> ground_superposition 
-          is_welltyped_on_subset[OF  wt_\<gamma> vars_conclusion'] 
+          C'_\<gamma> ground_superposition 
+          is_welltyped_on_subset[OF \<gamma>_is_welltyped vars_C'] 
           infinite_variables_per_type_\<V>\<^sub>3
-          typing(1, 2)
+          E_is_welltyped
+          D_is_welltyped
         unfolding ground.G_Inf_def \<iota>\<^sub>G
-        by(auto simp: typing renaming premise\<^sub>1_grounding premise\<^sub>2_grounding conclusion_grounding)
-        
+        using D_grounding E_grounding C_grounding
+        by(auto simp: \<V>\<^sub>1 \<V>\<^sub>2 \<rho>\<^sub>1 \<rho>\<^sub>2 rename_apart)
+
       then show ?thesis
         using is_inference_grounding_inference_groundings
         by blast
     qed
 
-    show "conclusion' \<cdot> \<gamma> = conclusion \<cdot> \<gamma>"
-      using conclusion'_\<gamma>.
+    show "C' \<cdot> \<gamma> = C \<cdot> \<gamma>"
+      using C'_\<gamma>.
   qed
 qed  
 
@@ -1665,7 +1500,7 @@ lemma eq_resolution_ground_instance:
     "\<iota>\<^sub>G \<in> ground.eq_resolution_inferences"
     "\<iota>\<^sub>G \<in> ground.Inf_from_q select\<^sub>G (\<Union>(clause_groundings ` N))"
     "subst_stability_on N"
-  obtains \<iota> where 
+  obtains \<iota> where
     "\<iota> \<in> Inf_from N" 
     "\<iota>\<^sub>G \<in> inference_groundings \<iota>"
 proof-
@@ -1769,9 +1604,9 @@ proof-
     "infinite_variables_per_type \<V>"
     using assms(2, 3) D\<^sub>G_in_groundings
     unfolding \<iota>\<^sub>G ground.Inf_from_q_def ground.Inf_from_def
-    (* TODO: *)
+      (* TODO: *)
     apply(elim ballE)
-     apply auto
+    apply auto
     by (metis clause.from_ground_inverse clause.ground_is_ground
         clause.obtain_grounding clause.subst_ident_if_ground
         select_ground_subst)
@@ -1830,37 +1665,37 @@ lemma superposition_ground_instance:
     "\<iota> \<in> Inf_from premises" 
     "\<iota>\<^sub>G \<in> inference_groundings \<iota>"
 proof-
-  obtain premise\<^sub>G\<^sub>1 premise\<^sub>G\<^sub>2 conclusion\<^sub>G where 
-    \<iota>\<^sub>G : "\<iota>\<^sub>G = Infer [premise\<^sub>G\<^sub>2, premise\<^sub>G\<^sub>1] conclusion\<^sub>G" and
-    superposition: "ground.superposition premise\<^sub>G\<^sub>2 premise\<^sub>G\<^sub>1 conclusion\<^sub>G"
+  obtain E\<^sub>G D\<^sub>G C\<^sub>G where 
+    \<iota>\<^sub>G : "\<iota>\<^sub>G = Infer [D\<^sub>G, E\<^sub>G] C\<^sub>G" and
+    superposition: "ground.superposition D\<^sub>G E\<^sub>G C\<^sub>G"
     using assms(1)
     by blast
 
   have 
-    premise\<^sub>G\<^sub>1_in_groundings: "premise\<^sub>G\<^sub>1 \<in> \<Union> (clause_groundings ` premises)" and  
-    premise\<^sub>G\<^sub>2_in_groundings: "premise\<^sub>G\<^sub>2 \<in> \<Union> (clause_groundings ` premises)"
+    E\<^sub>G_in_groundings: "E\<^sub>G \<in> \<Union> (clause_groundings ` premises)" and  
+    D\<^sub>G_in_groundings: "D\<^sub>G \<in> \<Union> (clause_groundings ` premises)"
     using assms(2)
     unfolding \<iota>\<^sub>G ground.Inf_from_q_def ground.Inf_from_def
     by simp_all
 
-  obtain premise\<^sub>1 \<V>\<^sub>1 premise\<^sub>2 \<V>\<^sub>2 \<gamma>\<^sub>1 \<gamma>\<^sub>2 where
-    premise\<^sub>1_\<gamma>\<^sub>1: "premise\<^sub>1 \<cdot> \<gamma>\<^sub>1 = clause.from_ground premise\<^sub>G\<^sub>1" and
-    premise\<^sub>2_\<gamma>\<^sub>2: "premise\<^sub>2 \<cdot> \<gamma>\<^sub>2 = clause.from_ground premise\<^sub>G\<^sub>2" and
+  obtain E \<V>\<^sub>1 D \<V>\<^sub>2 \<gamma>\<^sub>1 \<gamma>\<^sub>2 where
+    E_\<gamma>\<^sub>1: "E \<cdot> \<gamma>\<^sub>1 = clause.from_ground E\<^sub>G" and
+    D_\<gamma>\<^sub>2: "D \<cdot> \<gamma>\<^sub>2 = clause.from_ground D\<^sub>G" and
     select: 
-    "clause.from_ground (select\<^sub>G (clause.to_ground (premise\<^sub>1 \<cdot> \<gamma>\<^sub>1))) = select premise\<^sub>1 \<cdot> \<gamma>\<^sub>1"
-    "clause.from_ground (select\<^sub>G (clause.to_ground (premise\<^sub>2 \<cdot> \<gamma>\<^sub>2))) = select premise\<^sub>2 \<cdot> \<gamma>\<^sub>2" and
-    premise\<^sub>1_in_premises: "(premise\<^sub>1, \<V>\<^sub>1) \<in> premises" and
-    premise\<^sub>2_in_premises: "(premise\<^sub>2, \<V>\<^sub>2) \<in> premises" and 
+    "clause.from_ground (select\<^sub>G (clause.to_ground (E \<cdot> \<gamma>\<^sub>1))) = select E \<cdot> \<gamma>\<^sub>1"
+    "clause.from_ground (select\<^sub>G (clause.to_ground (D \<cdot> \<gamma>\<^sub>2))) = select D \<cdot> \<gamma>\<^sub>2" and
+    E_in_premises: "(E, \<V>\<^sub>1) \<in> premises" and
+    D_in_premises: "(D, \<V>\<^sub>2) \<in> premises" and 
     wt: 
-    "is_welltyped_on (clause.vars premise\<^sub>1) \<V>\<^sub>1 \<gamma>\<^sub>1"
-    "is_welltyped_on (clause.vars premise\<^sub>2) \<V>\<^sub>2 \<gamma>\<^sub>2"
+    "is_welltyped_on (clause.vars E) \<V>\<^sub>1 \<gamma>\<^sub>1"
+    "is_welltyped_on (clause.vars D) \<V>\<^sub>2 \<gamma>\<^sub>2"
     (*"term_subst.is_ground_subst \<gamma>\<^sub>1"
     "term_subst.is_ground_subst \<gamma>\<^sub>2" *)
-    "clause.is_welltyped \<V>\<^sub>1 premise\<^sub>1"
-    "clause.is_welltyped \<V>\<^sub>2 premise\<^sub>2"
+    "clause.is_welltyped \<V>\<^sub>1 E"
+    "clause.is_welltyped \<V>\<^sub>2 D"
     "infinite_variables_per_type \<V>\<^sub>1" 
     "infinite_variables_per_type \<V>\<^sub>2" 
-    using assms(2, 4) premise\<^sub>G\<^sub>1_in_groundings premise\<^sub>G\<^sub>2_in_groundings
+    using assms(2, 4) E\<^sub>G_in_groundings D\<^sub>G_in_groundings
     unfolding \<iota>\<^sub>G ground.Inf_from_q_def ground.Inf_from_def
     by (smt (verit) clause.from_ground_inverse clause.ground_is_ground clause.obtain_grounding select_ground_subst
         split_beta split_pairs)
@@ -1869,14 +1704,14 @@ proof-
     renaming: 
     "term_subst.is_renaming \<rho>\<^sub>1" 
     "term_subst.is_renaming \<rho>\<^sub>2"
-    "\<rho>\<^sub>1 ` (clause.vars premise\<^sub>1) \<inter> \<rho>\<^sub>2 ` (clause.vars premise\<^sub>2) = {}" and
+    "\<rho>\<^sub>1 ` (clause.vars E) \<inter> \<rho>\<^sub>2 ` (clause.vars D) = {}" and
     wt_\<rho>: 
-    "is_welltyped_on (clause.vars premise\<^sub>1) \<V>\<^sub>1 \<rho>\<^sub>1"
-    "is_welltyped_on (clause.vars premise\<^sub>2) \<V>\<^sub>2 \<rho>\<^sub>2"
+    "is_welltyped_on (clause.vars E) \<V>\<^sub>1 \<rho>\<^sub>1"
+    "is_welltyped_on (clause.vars D) \<V>\<^sub>2 \<rho>\<^sub>2"
     using welltyped.obtain_typed_renamings[OF infinite_UNIV _ _ wt(5,6)[unfolded infinite_variables_per_type_def, rule_format]] 
     by (metis clause.finite_vars(1))
 
-  have renaming_distinct: "clause.vars (premise\<^sub>1 \<cdot> \<rho>\<^sub>1) \<inter> clause.vars (premise\<^sub>2 \<cdot> \<rho>\<^sub>2) = {}"
+  have renaming_distinct: "clause.vars (E \<cdot> \<rho>\<^sub>1) \<inter> clause.vars (D \<cdot> \<rho>\<^sub>2) = {}"
     using renaming(3)
     unfolding renaming(1,2)[THEN clause.renaming_variables, symmetric]
     by blast
@@ -1887,31 +1722,31 @@ proof-
     unfolding term_subst.is_renaming_def
     by blast
 
-  have "select premise\<^sub>1 \<subseteq># premise\<^sub>1" "select premise\<^sub>2 \<subseteq># premise\<^sub>2"
+  have "select E \<subseteq># E" "select D \<subseteq># D"
     by (simp_all add: select_subset)
 
   then have select_subset: 
-    "select premise\<^sub>1 \<cdot> \<rho>\<^sub>1 \<subseteq># premise\<^sub>1 \<cdot> \<rho>\<^sub>1" 
-    "select premise\<^sub>2 \<cdot> \<rho>\<^sub>2 \<subseteq># premise\<^sub>2 \<cdot> \<rho>\<^sub>2"
+    "select E \<cdot> \<rho>\<^sub>1 \<subseteq># E \<cdot> \<rho>\<^sub>1" 
+    "select D \<cdot> \<rho>\<^sub>2 \<subseteq># D \<cdot> \<rho>\<^sub>2"
     by (simp_all add: image_mset_subseteq_mono clause.subst_def)
 
   define \<gamma> where 
     \<gamma>: "\<And>var. \<gamma> var \<equiv>
-          if var \<in> clause.vars (premise\<^sub>1 \<cdot> \<rho>\<^sub>1)
+          if var \<in> clause.vars (E \<cdot> \<rho>\<^sub>1)
           then (\<rho>\<^sub>1_inv \<odot> \<gamma>\<^sub>1) var 
           else (\<rho>\<^sub>2_inv \<odot> \<gamma>\<^sub>2) var"
 
-  have \<gamma>\<^sub>1: "\<forall>x\<in> clause.vars premise\<^sub>1. (\<rho>\<^sub>1 \<odot> \<gamma>) x = \<gamma>\<^sub>1 x"
+  have \<gamma>\<^sub>1: "\<forall>x\<in> clause.vars E. (\<rho>\<^sub>1 \<odot> \<gamma>) x = \<gamma>\<^sub>1 x"
   proof(intro ballI)
     fix x
-    assume x_in_vars: "x \<in> clause.vars premise\<^sub>1"
+    assume x_in_vars: "x \<in> clause.vars E"
 
     obtain y where y: "\<rho>\<^sub>1 x = Var y"
       by (meson is_Var_def renaming(1) term_subst_is_renaming_iff)
 
-    then have "y \<in> clause.vars (premise\<^sub>1 \<cdot> \<rho>\<^sub>1)"
+    then have "y \<in> clause.vars (E \<cdot> \<rho>\<^sub>1)"
       using x_in_vars renaming(1) clause.renaming_variables by fastforce
-    
+
 
     then have "\<gamma> y = \<rho>\<^sub>1_inv y \<cdot>t \<gamma>\<^sub>1"
       by (simp add: \<gamma> subst_compose)
@@ -1920,15 +1755,15 @@ proof-
       by (metis y \<rho>\<^sub>1_inv eval_term.simps(1) subst_compose)
   qed
 
-  have \<gamma>\<^sub>2: "\<forall>x\<in> clause.vars premise\<^sub>2. (\<rho>\<^sub>2 \<odot> \<gamma>) x = \<gamma>\<^sub>2 x"
+  have \<gamma>\<^sub>2: "\<forall>x\<in> clause.vars D. (\<rho>\<^sub>2 \<odot> \<gamma>) x = \<gamma>\<^sub>2 x"
   proof(intro ballI)
     fix x
-    assume x_in_vars: "x \<in> clause.vars premise\<^sub>2"
+    assume x_in_vars: "x \<in> clause.vars D"
 
     obtain y where y: "\<rho>\<^sub>2 x = Var y"
       by (meson is_Var_def renaming(2) term_subst_is_renaming_iff)
 
-    then have "y \<in> clause.vars (premise\<^sub>2 \<cdot> \<rho>\<^sub>2)"
+    then have "y \<in> clause.vars (D \<cdot> \<rho>\<^sub>2)"
       using x_in_vars renaming(2) clause.renaming_variables by fastforce
 
     then have "\<gamma> y = \<rho>\<^sub>2_inv y \<cdot>t \<gamma>\<^sub>2"
@@ -1938,21 +1773,21 @@ proof-
       by (metis y \<rho>\<^sub>2_inv eval_term.simps(1) subst_compose)
   qed
 
-  have \<gamma>\<^sub>1_is_ground: "\<forall>x\<in>clause.vars premise\<^sub>1. term.is_ground (\<gamma>\<^sub>1 x)"
+  have \<gamma>\<^sub>1_is_ground: "\<forall>x\<in>clause.vars E. term.is_ground (\<gamma>\<^sub>1 x)"
     by (metis clause.ground_is_ground clause.variable_grounding
-        premise\<^sub>1_\<gamma>\<^sub>1)
-    
-  have \<gamma>\<^sub>2_is_ground: "\<forall>x\<in>clause.vars premise\<^sub>2. term.is_ground (\<gamma>\<^sub>2 x)"
+        E_\<gamma>\<^sub>1)
+
+  have \<gamma>\<^sub>2_is_ground: "\<forall>x\<in>clause.vars D. term.is_ground (\<gamma>\<^sub>2 x)"
     by (metis clause.ground_is_ground clause.variable_grounding
-        premise\<^sub>2_\<gamma>\<^sub>2)
+        D_\<gamma>\<^sub>2)
 
   have wt_\<gamma>:
-    "is_welltyped_on (clause.vars premise\<^sub>1) \<V>\<^sub>1 (\<rho>\<^sub>1 \<odot> \<gamma>)"
-    "is_welltyped_on (clause.vars premise\<^sub>2) \<V>\<^sub>2 (\<rho>\<^sub>2 \<odot> \<gamma>)"
+    "is_welltyped_on (clause.vars E) \<V>\<^sub>1 (\<rho>\<^sub>1 \<odot> \<gamma>)"
+    "is_welltyped_on (clause.vars D) \<V>\<^sub>2 (\<rho>\<^sub>2 \<odot> \<gamma>)"
     using wt(1,2) is_welltyped_on_subset \<gamma>\<^sub>1 \<gamma>\<^sub>2
     by auto    
 
-  (*have "term_subst.is_ground_subst (\<rho>\<^sub>1_inv \<odot> \<gamma>\<^sub>1)" "term_subst.is_ground_subst (\<rho>\<^sub>2_inv \<odot> \<gamma>\<^sub>2)"
+(*have "term_subst.is_ground_subst (\<rho>\<^sub>1_inv \<odot> \<gamma>\<^sub>1)" "term_subst.is_ground_subst (\<rho>\<^sub>2_inv \<odot> \<gamma>\<^sub>2)"
     using term_subst.is_ground_subst_comp_right wt by blast+
 
   then have is_ground_subst_\<gamma>: "term_subst.is_ground_subst \<gamma>"
@@ -1960,31 +1795,32 @@ proof-
     using is_ground_subst_if
     by fast*)
 
-  have premise\<^sub>1_\<gamma>: "premise\<^sub>1 \<cdot> \<rho>\<^sub>1 \<cdot> \<gamma> = clause.from_ground premise\<^sub>G\<^sub>1" 
+  have E_\<gamma>: "E \<cdot> \<rho>\<^sub>1 \<odot> \<gamma> = clause.from_ground E\<^sub>G" 
   proof -
-    have "premise\<^sub>1 \<cdot> \<rho>\<^sub>1 \<odot> (\<rho>\<^sub>1_inv \<odot> \<gamma>\<^sub>1) = clause.from_ground premise\<^sub>G\<^sub>1"
-      by (metis \<rho>\<^sub>1_inv premise\<^sub>1_\<gamma>\<^sub>1 subst_monoid_mult.mult.left_neutral subst_monoid_mult.mult_assoc)
+    have "E \<cdot> \<rho>\<^sub>1 \<odot> (\<rho>\<^sub>1_inv \<odot> \<gamma>\<^sub>1) = clause.from_ground E\<^sub>G"
+      by (metis \<rho>\<^sub>1_inv E_\<gamma>\<^sub>1 subst_monoid_mult.mult.left_neutral subst_monoid_mult.mult_assoc)
 
     then show ?thesis
-      using \<gamma>\<^sub>1 premise\<^sub>1_\<gamma>\<^sub>1 clause.subst_eq by fastforce
+      using \<gamma>\<^sub>1 E_\<gamma>\<^sub>1 clause.subst_eq by fastforce
   qed
 
-  have premise\<^sub>2_\<gamma>: "premise\<^sub>2 \<cdot> \<rho>\<^sub>2 \<cdot> \<gamma> = clause.from_ground premise\<^sub>G\<^sub>2" 
+  have D_\<gamma>: "D \<cdot> \<rho>\<^sub>2 \<odot>  \<gamma> = clause.from_ground D\<^sub>G" 
   proof -
-    have "premise\<^sub>2 \<cdot> \<rho>\<^sub>2 \<odot> (\<rho>\<^sub>2_inv \<odot> \<gamma>\<^sub>2) = clause.from_ground premise\<^sub>G\<^sub>2"
-      by (metis \<rho>\<^sub>2_inv premise\<^sub>2_\<gamma>\<^sub>2 subst_monoid_mult.mult.left_neutral subst_monoid_mult.mult_assoc)
+    have "D \<cdot> \<rho>\<^sub>2 \<odot> (\<rho>\<^sub>2_inv \<odot> \<gamma>\<^sub>2) = clause.from_ground D\<^sub>G"
+      by (metis \<rho>\<^sub>2_inv D_\<gamma>\<^sub>2 subst_monoid_mult.mult.left_neutral subst_monoid_mult.mult_assoc)
 
     then show ?thesis
-      using \<gamma>\<^sub>2 premise\<^sub>2_\<gamma>\<^sub>2 clause.subst_eq
+      using \<gamma>\<^sub>2 D_\<gamma>\<^sub>2 clause.subst_eq
       by fastforce
   qed
 
-  have "premise\<^sub>1 \<cdot> \<rho>\<^sub>1 \<cdot> \<gamma> = premise\<^sub>1 \<cdot> \<gamma>\<^sub>1"
-    by (simp add: premise\<^sub>1_\<gamma> premise\<^sub>1_\<gamma>\<^sub>1)
+  have "E \<cdot> \<rho>\<^sub>1 \<odot> \<gamma> = E \<cdot> \<gamma>\<^sub>1"
+    using E_\<gamma> E_\<gamma>\<^sub>1 
+    by argo
 
-  moreover have "select premise\<^sub>1 \<cdot> \<rho>\<^sub>1 \<cdot> \<gamma> = select premise\<^sub>1 \<cdot> \<gamma>\<^sub>1"
+  moreover have "select E \<cdot> \<rho>\<^sub>1 \<cdot> \<gamma> = select E \<cdot> \<gamma>\<^sub>1"
   proof-
-    have "clause.vars (select premise\<^sub>1 \<cdot> \<rho>\<^sub>1) \<subseteq> clause.vars (premise\<^sub>1 \<cdot> \<rho>\<^sub>1)"
+    have "clause.vars (select E \<cdot> \<rho>\<^sub>1) \<subseteq> clause.vars (E \<cdot> \<rho>\<^sub>1)"
       using select_subset(1) clause_submset_vars_clause_subset by blast
 
     then show ?thesis
@@ -1995,81 +1831,83 @@ proof-
   qed
 
   ultimately have select\<^sub>1: 
-    "clause.from_ground (select\<^sub>G (clause.to_ground (premise\<^sub>1 \<cdot> \<rho>\<^sub>1 \<cdot> \<gamma>))) = select premise\<^sub>1 \<cdot> \<rho>\<^sub>1 \<cdot> \<gamma>"
+    "clause.from_ground (select\<^sub>G (clause.to_ground (E \<cdot> \<rho>\<^sub>1 \<odot> \<gamma>))) = select E \<cdot> \<rho>\<^sub>1 \<odot> \<gamma>"
     using select(1)
-    by argo
-  
-  have "premise\<^sub>2 \<cdot> \<rho>\<^sub>2 \<cdot> \<gamma> = premise\<^sub>2 \<cdot> \<gamma>\<^sub>2"
-    by (simp add: premise\<^sub>2_\<gamma> premise\<^sub>2_\<gamma>\<^sub>2)
+    by auto
 
-  moreover have "select premise\<^sub>2 \<cdot> \<rho>\<^sub>2 \<cdot> \<gamma> = select premise\<^sub>2 \<cdot> \<gamma>\<^sub>2"
-   proof-
-    have "clause.vars (select premise\<^sub>2 \<cdot> \<rho>\<^sub>2) \<subseteq> clause.vars (premise\<^sub>2 \<cdot> \<rho>\<^sub>2)"
+  have "D \<cdot> \<rho>\<^sub>2 \<odot> \<gamma> = D \<cdot> \<gamma>\<^sub>2"
+    using D_\<gamma> D_\<gamma>\<^sub>2
+    by simp
+
+  moreover have "select D \<cdot> \<rho>\<^sub>2 \<odot> \<gamma> = select D \<cdot> \<gamma>\<^sub>2"
+  proof-
+    have "clause.vars (select D \<cdot> \<rho>\<^sub>2) \<subseteq> clause.vars (D \<cdot> \<rho>\<^sub>2)"
       using select_subset(2) clause_submset_vars_clause_subset by blast
 
     then show ?thesis
       unfolding \<gamma> 
-      by (smt (verit, best) \<gamma>\<^sub>2 \<gamma> \<open>select premise\<^sub>2 \<subseteq># premise\<^sub>2\<close> clause_submset_vars_clause_subset
+      by (smt (verit, best) \<gamma>\<^sub>2 \<gamma> \<open>select D \<subseteq># D\<close> clause_submset_vars_clause_subset
           clause.subst_eq subset_iff clause.comp_subst.left.monoid_action_compatibility)
   qed
 
   ultimately have select\<^sub>2: 
-    "clause.from_ground (select\<^sub>G (clause.to_ground (premise\<^sub>2 \<cdot> \<rho>\<^sub>2 \<cdot> \<gamma>))) = select premise\<^sub>2 \<cdot> \<rho>\<^sub>2 \<cdot> \<gamma>"   
+    "clause.from_ground (select\<^sub>G (clause.to_ground (D \<cdot> \<rho>\<^sub>2 \<odot> \<gamma>))) = select D \<cdot> \<rho>\<^sub>2 \<odot> \<gamma>"   
     using select(2) 
     by argo
 
-  obtain "conclusion" where 
-    conclusion_\<gamma>: "conclusion \<cdot> \<gamma> = clause.from_ground conclusion\<^sub>G"
+  obtain C where 
+    C_\<gamma>: "C \<cdot> \<gamma> = clause.from_ground C\<^sub>G"
     by (meson clause.ground_is_ground clause.subst_ident_if_ground)
 
   then have 
-    premise\<^sub>1_grounding: "clause.is_ground (premise\<^sub>1 \<cdot> \<rho>\<^sub>1 \<cdot> \<gamma>)" and 
-    premise\<^sub>2_grounding: "clause.is_ground (premise\<^sub>2 \<cdot> \<rho>\<^sub>2 \<cdot> \<gamma>)" and 
-    premise\<^sub>G\<^sub>1: "premise\<^sub>G\<^sub>1 = clause.to_ground (premise\<^sub>1 \<cdot> \<rho>\<^sub>1 \<cdot> \<gamma>)" and 
-    premise\<^sub>G\<^sub>2: "premise\<^sub>G\<^sub>2 = clause.to_ground (premise\<^sub>2 \<cdot> \<rho>\<^sub>2 \<cdot> \<gamma>)" and 
-    conclusion_grounding: "clause.is_ground (conclusion \<cdot> \<gamma>)" and
-    conclusion\<^sub>G: "conclusion\<^sub>G = clause.to_ground (conclusion \<cdot> \<gamma>)"
-    by (simp_all add: premise\<^sub>1_\<gamma> premise\<^sub>2_\<gamma>)
+    E_grounding: "clause.is_ground (E \<cdot> \<rho>\<^sub>1 \<odot> \<gamma>)" and 
+    D_grounding: "clause.is_ground (D \<cdot> \<rho>\<^sub>2 \<odot> \<gamma>)" and 
+    E\<^sub>G: "E\<^sub>G = clause.to_ground (E \<cdot> \<rho>\<^sub>1 \<odot> \<gamma>)" and 
+    D\<^sub>G: "D\<^sub>G = clause.to_ground (D \<cdot> \<rho>\<^sub>2 \<odot> \<gamma>)" and 
+    C_grounding: "clause.is_ground (C \<cdot> \<gamma>)" and
+    C\<^sub>G: "C\<^sub>G = clause.to_ground (C \<cdot> \<gamma>)"
+    using E_\<gamma> D_\<gamma>
+    by simp_all
 
-  have "clause_groundings (premise\<^sub>1, \<V>\<^sub>1) \<union> clause_groundings (premise\<^sub>2, \<V>\<^sub>2)
+  have "clause_groundings (E, \<V>\<^sub>1) \<union> clause_groundings (D, \<V>\<^sub>2)
      \<subseteq> \<Union> (clause_groundings ` premises)"
-    using premise\<^sub>1_in_premises premise\<^sub>2_in_premises by blast
+    using E_in_premises D_in_premises by blast
 
   then have \<iota>\<^sub>G_not_redunant:
-    "\<iota>\<^sub>G \<notin> ground.GRed_I (clause_groundings (premise\<^sub>1, \<V>\<^sub>1) \<union> clause_groundings (premise\<^sub>2, \<V>\<^sub>2))"
+    "\<iota>\<^sub>G \<notin> ground.GRed_I (clause_groundings (E, \<V>\<^sub>1) \<union> clause_groundings (D, \<V>\<^sub>2))"
     using assms(3) ground.Red_I_of_subset
     by blast
 
-  then obtain conclusion' \<V>\<^sub>3 where 
-    superposition: "superposition (premise\<^sub>2, \<V>\<^sub>2) (premise\<^sub>1, \<V>\<^sub>1) (conclusion', \<V>\<^sub>3)" and
+  then obtain C' \<V>\<^sub>3 where 
+    superposition: "superposition (D, \<V>\<^sub>2) (E, \<V>\<^sub>1) (C', \<V>\<^sub>3)" and
     inference_groundings: 
-      "\<iota>\<^sub>G \<in> inference_groundings (Infer [(premise\<^sub>2, \<V>\<^sub>2), (premise\<^sub>1, \<V>\<^sub>1)] (conclusion', \<V>\<^sub>3))" and  
-    conclusion'_\<gamma>_conclusion_\<gamma>: "conclusion' \<cdot> \<gamma> = conclusion \<cdot> \<gamma>"
+    "\<iota>\<^sub>G \<in> inference_groundings (Infer [(D, \<V>\<^sub>2), (E, \<V>\<^sub>1)] (C', \<V>\<^sub>3))" and  
+    C'_\<gamma>_C_\<gamma>: "C' \<cdot> \<gamma> = C \<cdot> \<gamma>"
     using 
       superposition_lifting[OF 
+        superposition[unfolded  D\<^sub>G E\<^sub>G C\<^sub>G]
         renaming(1,2)
         renaming_distinct
-        premise\<^sub>1_grounding 
-        premise\<^sub>2_grounding 
-        conclusion_grounding
+        E_grounding 
+        D_grounding 
+        C_grounding
         select\<^sub>1
         select\<^sub>2
-        superposition[unfolded  premise\<^sub>G\<^sub>2 premise\<^sub>G\<^sub>1 conclusion\<^sub>G]
-        \<iota>\<^sub>G_not_redunant[unfolded \<iota>\<^sub>G premise\<^sub>G\<^sub>2 premise\<^sub>G\<^sub>1 conclusion\<^sub>G]
         wt(3, 4)
         wt_\<gamma>
         wt_\<rho>
         wt(5, 6)
+        \<iota>\<^sub>G_not_redunant[unfolded \<iota>\<^sub>G D\<^sub>G E\<^sub>G C\<^sub>G]
         ]
-    unfolding \<iota>\<^sub>G conclusion\<^sub>G premise\<^sub>G\<^sub>1 premise\<^sub>G\<^sub>2 
+    unfolding \<iota>\<^sub>G C\<^sub>G E\<^sub>G D\<^sub>G 
     by blast
 
-  let ?\<iota> = "Infer [(premise\<^sub>2, \<V>\<^sub>2), (premise\<^sub>1, \<V>\<^sub>1)] (conclusion', \<V>\<^sub>3)"
+  let ?\<iota> = "Infer [(D, \<V>\<^sub>2), (E, \<V>\<^sub>1)] (C', \<V>\<^sub>3)"
 
   show ?thesis
   proof(rule that)
     show "?\<iota> \<in> Inf_from premises"
-      using premise\<^sub>1_in_premises premise\<^sub>2_in_premises superposition
+      using E_in_premises D_in_premises superposition
       unfolding Inf_from_def inferences_def inference_system.Inf_from_def
       by auto
 
